Large refactoring
Move extensionality lemmas proved for forall deduction to
Denotational, prove irrel and _change_pf from this
Remove some uneeded lemmas and reorganize Denotational to generalize
Push changes through
Create Logic.v for metatheorems about why3 logic
Create Shallow.v for shallow embedding theorems
Create NatDed.v for natural deduction, delete old code

proofs/core/Denotational.v
@@ -43,7 +43,21 @@ Definition proj2' {A B: Prop} (H: A /\ B) : B :=
   | conj x x0 => x0
   end.
 
-Section Denot.
+(*Useful for [match_val_single]*)
+Ltac case_find_constr :=
+  repeat match goal with
+  | |- context [match funsym_eq_dec (projT1 ?x) ?f with 
+    | left Heq => _ | right Hneq => _ end] =>
+      generalize dependent x
+  end. 
+
+(*First, we give the definitions, and then we prove properties
+  of these definitions.
+  We need to be very careful about which variables are generic
+  and which are fixed in Sections.
+*)
+
+Section DenotDef.
 
 Context {gamma: context} (gamma_valid: valid_context gamma)
   (pd: pi_dom) .
@@ -137,169 +151,6 @@ Proof.
         (Nat.succ_inj (length ts) (length atl) Hlents)
         (Forall_inv_tail Hall)))).
 Defined.
-
-(*If the reps are equal only for the terms in the list,
-  then the arg_lists are equal, and they are irrelevant
-  in the choice of proof*)
-
-(*We prove a very general extensionality lemma that allows us
-  to modify the val_typevar, val_vars, reps, and proofs.
-  We give specialized versions below*)
-Lemma get_arg_list_vt_ext (vt1 vt2: val_typevar) (s: fpsym)
-(vs: list vty) (ts1 ts2: list term) vv1 vv2 pf
-(reps1 reps2: forall (vt: val_typevar) (pf: pi_funpred gamma_valid pd) 
-  (vv: val_vars pd vt)
-  (t: term) (ty: vty) (Hty: term_has_type gamma t ty),
-  domain (v_subst vt ty))
-(Hts: length ts1 = length ts2)
-(Hreps: forall (i: nat),
-  i < length ts1 ->
-  forall (ty: vty) Hty1 Hty2 Heq,
-    dom_cast (dom_aux pd) Heq 
-      (reps1 vt1 pf vv1 (nth i ts1 tm_d) ty Hty1) =
-    reps2 vt2 pf vv2 (nth i ts2 tm_d) ty Hty2)
-{args: list vty}
-(Hlents1: length ts1 = length args)
-(Hlents2: length ts2 = length args)
-(Hlenvs1 Hlenvs2: length vs = length (s_params s))
-(Hall1: Forall (fun x => term_has_type gamma (fst x) (snd x))
-  (combine ts1 (map (ty_subst (s_params s) vs) args)))
-(Hall2: Forall (fun x => term_has_type gamma (fst x) (snd x))
-  (combine ts2 (map (ty_subst (s_params s) vs) args)))
-(Heq: map (v_subst vt2) vs = map (v_subst vt1) vs):
-cast_arg_list 
-  (f_equal (fun x => ty_subst_list_s (s_params s) x args) (eq_sym Heq))
-  (get_arg_list vt1 s vs ts1 (reps1 vt1 pf vv1) Hlents1 Hlenvs1 Hall1) =
-get_arg_list vt2 s vs ts2 (reps2 vt2 pf vv2) Hlents2 Hlenvs2 Hall2.
-Proof.
-  generalize dependent (f_equal (fun x : list sort => ty_subst_list_s (s_params s) x args) (eq_sym Heq)).
-  clear Heq.
-  unfold get_arg_list. simpl.
-  assert (Hlenvs1 = Hlenvs2). apply UIP_dec. apply Nat.eq_dec.
-  subst.
-  generalize dependent args.
-  generalize dependent ts2. 
-  induction ts1; simpl; intros. 
-  - destruct ts2; [|subst; inversion Hts].
-    destruct args; simpl; auto; [|inversion Hlents1].
-    assert (e = eq_refl). apply UIP_dec. apply list_eq_dec.
-    apply sort_eq_dec. 
-    subst. reflexivity.
-  - destruct ts2; inversion Hts.
-    destruct args.
-    + inversion Hlents2.
-    + simpl in Hlenvs2. simpl.
-      simpl in e.
-      rewrite (cast_arg_list_cons e).
-      f_equal.
-      * rewrite rewrite_dom_cast, !dom_cast_compose.
-        erewrite <- (Hreps 0) with(Hty1:=Forall_inv Hall1) (Heq:=
-        (eq_trans 
-          ((eq_trans (funsym_subst_eq (s_params s) vs vt1 v (s_params_Nodup s) (eq_sym Hlenvs2))
-          (cons_inj_hd e)))
-          (eq_sym ((funsym_subst_eq (s_params s) vs vt2 v (s_params_Nodup s) (eq_sym Hlenvs2)))))
-        ); try lia.
-        rewrite !dom_cast_compose. apply dom_cast_eq.
-      * apply IHts1; auto.
-        intros i Hi ty Hty1 Hty2 Heq.
-        apply (Hreps (S i) (ltac:(lia))).
-Qed.
-
-(*Specialized versions of the above: TODO: remove some of them,
-  legacy*)
-Lemma get_arg_list_vt_eq (vt1 vt2: val_typevar) (s: fpsym)
-(vs: list vty) (ts: list term) vv1 vv2 pf
-(reps: forall (vt: val_typevar) (pf: pi_funpred gamma_valid pd) 
-  (vv: val_vars pd vt)
-  (t: term) (ty: vty) (Hty: term_has_type gamma t ty),
-  domain (v_subst vt ty))
-(Hreps: Forall
-  (fun tm : term =>
-    forall (ty: vty) (Hty1 Hty2: term_has_type gamma tm ty) 
-      (Heq: v_subst vt2 ty = v_subst vt1 ty),
-      reps vt1 pf vv1 tm ty Hty1 =
-      dom_cast (dom_aux pd) Heq (reps vt2 pf vv2 tm ty Hty2)
-    ) ts)
-Hlents Hlenvs Hall
-(Heq: map (v_subst vt2) vs = map (v_subst vt1) vs):
-cast_arg_list (f_equal (sym_sigma_args s) (eq_sym Heq))
-  (get_arg_list vt1 s vs ts (reps vt1 pf vv1) Hlents Hlenvs Hall) =
-get_arg_list vt2 s vs ts (reps vt2 pf vv2) Hlents Hlenvs Hall.
-Proof.
-  apply get_arg_list_vt_ext; auto. 
-  rewrite Forall_forall in Hreps.
-  intros.
-  symmetry. rewrite Hreps with(Heq:=eq_sym Heq0)(Hty2:=Hty2).
-  rewrite !dom_cast_twice. reflexivity.
-  apply nth_In. auto.
-Qed. 
-
-(*TODO: shouldn't need this and the below*)
-(*easier to prove this directly, since reps is handled differently,
-  should really unify*)
-Lemma get_arg_list_ext (v: val_typevar)
-  (s: fpsym) (vs: list vty) (ts1 ts2: list term) 
-  (reps1 reps2: forall (t: term) (ty: vty),
-    term_has_type gamma t ty ->
-    domain (val v ty))
-  (Hts: length ts1 = length ts2)
-  (Hreps: forall (i: nat),
-    i < length ts1 ->
-    forall (ty : vty) Hty1 Hty2,
-    reps1 (nth i ts1 tm_d) ty Hty1 = reps2 (nth i ts2 tm_d) ty Hty2)
-  {args: list vty}
-  (Hlents1: length ts1 = length args)
-  (Hlents2: length ts2 = length args)
-  (Hlenvs1 Hlenvs2: length vs = length (s_params s))
-  (Hall1: Forall (fun x => term_has_type gamma (fst x) (snd x))
-    (combine ts1 (map (ty_subst (s_params s) vs) args)))
-  (Hall2: Forall (fun x => term_has_type gamma (fst x) (snd x))
-    (combine ts2 (map (ty_subst (s_params s) vs) args))):
-  get_arg_list v s vs ts1 reps1 Hlents1 Hlenvs1 Hall1 =
-  get_arg_list v s vs ts2 reps2 Hlents2 Hlenvs2 Hall2.
-Proof.
-  unfold get_arg_list. simpl.
-  assert (Hlenvs1 = Hlenvs2). apply UIP_dec. apply Nat.eq_dec.
-  subst.
-  generalize dependent args.
-  generalize dependent ts2. 
-  induction ts1; simpl; intros. 
-  - destruct ts2; [|subst; inversion Hts].
-    destruct args; auto. inversion Hlents1.
-  - destruct ts2; inversion Hts.
-    destruct args.
-    + inversion Hlents2.
-    + simpl in Hlenvs2. simpl. f_equal.
-      * f_equal.
-        apply (Hreps 0). lia.
-      * apply IHts1; auto.
-        intros j Hj ty Hty1 Hty2.
-        apply (Hreps (S j)); lia.
-Qed.
-
-(*A corollary when ts are equal*)
-Lemma get_arg_list_eq (v: val_typevar)
-(s: fpsym) (vs: list vty) (ts: list term) 
-(reps1 reps2: forall (t: term) (ty: vty),
-  term_has_type gamma t ty ->
-  domain (val v ty))
-(Hreps: Forall
-(fun tm : term =>
- forall (ty : vty) (Hty1 Hty2: term_has_type gamma tm ty),
- reps1 tm ty Hty1 = reps2 tm ty Hty2) ts)
-{args: list vty}
-(Hlents1 Hlents2: length ts = length args)
-(Hlenvs1 Hlenvs2: length vs = length (s_params s))
-(Hall1 Hall2: Forall (fun x => term_has_type gamma (fst x) (snd x))
-  (combine ts (map (ty_subst (s_params s) vs) args))):
-get_arg_list v s vs ts reps1 Hlents1 Hlenvs1 Hall1 =
-get_arg_list v s vs ts reps2 Hlents2 Hlenvs2 Hall2.
-Proof.
-  apply get_arg_list_ext; auto.
-  intros i Hi ty H1 H2.
-  rewrite Forall_forall in Hreps; apply Hreps.
-  apply nth_In; auto.
-Qed.
 
 (*The function version*)
 
@@ -507,18 +358,6 @@ Proof.
   intros. inversion H; subst. auto.
 Qed.
 
-(*TOOD: move*)
-Lemma v_subst_cons {f} ts vs:
-  v_subst f (vty_cons ts vs) =
-  typesym_to_sort ts (map (v_subst f) vs).
-Proof.
-  apply sort_inj. simpl.
-  f_equal. apply list_eq_ext'; rewrite !map_length; auto.
-  intros n d Hn.
-  rewrite !map_nth_inbound with (d2:=s_int); [|rewrite map_length; auto].
-  rewrite !map_nth_inbound with (d2:=vty_int); auto.
-Qed.
-
 (*Typecast we need for inner arg list*)
 Lemma sym_sigma_args_map (v: val_typevar) (f: funsym) 
   (vs: list vty):
@@ -590,10 +429,7 @@ Proof.
 Qed.
 
 Definition cast_prop {A: Set} (P: A -> Prop) {a1 a2: A} (H: a1 = a2)
-  (Hp: P a1) : P a2 :=
-  match H with
-  |eq_refl => Hp
-  end.
+  (Hp: P a1) : P a2 := eq_ind _ P Hp _ H.
 
 Definition pat_has_type_eq {s p ty1 ty2} (H: ty1 = ty2) 
   (Hp: pattern_has_type s p ty1):
@@ -893,31 +729,10 @@ Proof.
   destruct (Hadtspec m adt vs2 eq_refl)
     as [Htyeq [Hinmut Hinctx]].
   simpl.
-  destruct (funsym_eq_dec
-  (projT1
-      (find_constr_rep gamma_valid m Hinctx (map (val v) vs2)
-        (eq_trans (map_length (val v) vs2)
-            (Hvslen2 m adt vs2 eq_refl
-              (pat_has_type_valid gamma_valid (Pconstr f l l0) ty Hp)))
-        (dom_aux pd) adt Hinmut (adts pd m (map (val v) vs2)) 
-        (gamma_all_unif gamma_valid m Hinctx)
-        (scast (adts pd m (map (val v) vs2) adt Hinmut)
-            (dom_cast (dom_aux pd)
-              (eq_trans (f_equal (val v) Htyeq) (v_subst_cons (adt_name adt) vs2)) d))))
-  f); [|reflexivity]. 
   (*Need nested induction, simplify first*)
-  generalize dependent (find_constr_rep gamma_valid m Hinctx (map (val v) vs2)
-  (eq_trans (map_length (val v) vs2)
-      (Hvslen2 m adt vs2 eq_refl
-        (pat_has_type_valid gamma_valid (Pconstr f l l0) ty Hp)))
-  (dom_aux pd) adt Hinmut (adts pd m (map (val v) vs2)) 
-  (gamma_all_unif gamma_valid m Hinctx)
-  (scast (adts pd m (map (val v) vs2) adt Hinmut)
-      (dom_cast (dom_aux pd)
-        (eq_trans (f_equal (val v) Htyeq) (v_subst_cons (adt_name adt) vs2))
-        d))).
-  intros constr. destruct constr as [f' Hf']. simpl. intros Hf; subst.
-  simpl.
+  case_find_constr. intros.
+  destruct (funsym_eq_dec (projT1 s) f); [|reflexivity].
+  destruct s as [f' Hf']. simpl in *. subst. 
   match goal with 
   | |- ?f ?x1 ?x2 ?x3 ?x4 = ?g ?x1 ?x2 ?x3 ?x4 =>
     let H := fresh in
@@ -945,6 +760,7 @@ Qed.
 (*Now we want a generic way to prove things about
   [match_val_single] so we don't have to do all of the very
   tedious generalization and nested induction every time*)
+(*TODO: this is not very useful, we cannot use in many places*)
 Lemma match_val_single_ind 
 (P : forall (v : val_typevar) (ty : vty) (p : pattern)
   (d: domain (val v ty)),
@@ -1085,32 +901,14 @@ Proof.
     destruct (Hadtspec m adt vs2 eq_refl)
       as [Htyeq [Hinmut Hinctx]].
     simpl.
-    destruct (funsym_eq_dec
-    (projT1
-       (find_constr_rep gamma_valid m Hinctx (map (val v) vs2)
-          (eq_trans (map_length (val v) vs2)
-             (Hvslen2 m adt vs2 eq_refl
-                (pat_has_type_valid gamma_valid (Pconstr f vs ps) ty Hp)))
-          (dom_aux pd) adt Hinmut (adts pd m (map (val v) vs2)) 
-          (gamma_all_unif gamma_valid m Hinctx)
-          (scast (adts pd m (map (val v) vs2) adt Hinmut)
-             (dom_cast (dom_aux pd)
-                (eq_trans (f_equal (val v) Htyeq) (v_subst_cons (adt_name adt) vs2)) d))))
-    f).
-    2: {
-      apply (Hconstr2 v ty f vs ps Hp d m vs2 adt Hisadt Htyeq Hinmut _ _ n).
-    }
-    (*Need nested induction, simplify first*)
-    generalize dependent (find_constr_rep gamma_valid m Hinctx (map (val v) vs2)
-    (eq_trans (map_length (val v) vs2)
-       (Hvslen2 m adt vs2 eq_refl
-          (pat_has_type_valid gamma_valid (Pconstr f vs ps) ty Hp)))
-    (dom_aux pd) adt Hinmut (adts pd m (map (val v) vs2)) 
-    (gamma_all_unif gamma_valid m Hinctx)
-    (scast (adts pd m (map (val v) vs2) adt Hinmut)
-       (dom_cast (dom_aux pd)
-          (eq_trans (f_equal (val v) Htyeq) (v_subst_cons (adt_name adt) vs2))
-          d))).
+    match goal with
+    | |- context [match funsym_eq_dec (projT1 ?x) ?f with 
+      | left Heq => _ | right Hneq => _ end ] =>
+        destruct (funsym_eq_dec (projT1 x) f) ;[
+          generalize dependent x| 
+          apply (Hconstr2 v ty f vs ps Hp d m vs2 adt Hisadt Htyeq Hinmut _ _ n)
+        ]
+    end.
     intros constr. destruct constr as [f' Hf']. simpl. intros Hf; subst.
     simpl.
     match goal with
@@ -1188,96 +986,6 @@ Proof.
       * inversion H; subst. inversion Hty'; subst. reflexivity.
       * apply (IH _ eq_refl); auto.
     + inversion H.
-Qed.
-
-(*2. [match_val_single] is irrelevant in the typing proof*)
-Lemma match_val_single_irrel (v: val_typevar) (ty: vty)
-(p: pattern)
-(Hval1 Hval2: pattern_has_type gamma p ty)
-(d: domain (val v ty)) :
-  match_val_single v ty p Hval1 d =
-  match_val_single v ty p Hval2 d.
-Proof.
-  revert Hval1 Hval2. revert d. generalize dependent ty.
-  induction p; intros; auto.
-  - rewrite !match_val_single_rewrite; simpl.
-    (*The hard case: need lots of generalization for dependent types
-      and need nested induction*) 
-    generalize dependent (@is_vty_adt_some gamma ty).
-    generalize dependent (@adt_vty_length_eq gamma gamma_valid ty).
-    generalize dependent (@constr_length_eq ty).
-    destruct (is_vty_adt gamma ty) eqn : Hisadt; [|reflexivity].
-    intros Hvslen1 Hvslen2 Hadtspec.
-    destruct p as [[m adt] vs2].
-    destruct (Hadtspec m adt vs2 eq_refl)
-      as [Htyeq [Hinmut Hinctx]].
-    simpl.
-     (*This part is actually easy: all nat equality proofs are equal*)
-    generalize dependent (Hvslen2 m adt vs2 eq_refl
-    (pat_has_type_valid gamma_valid (Pconstr f vs ps) ty Hval1)).
-    generalize dependent (Hvslen2 m adt vs2 eq_refl
-    (pat_has_type_valid gamma_valid (Pconstr f vs ps) ty Hval2)).
-    intros.
-    assert (e = e0) by (apply UIP_dec, Nat.eq_dec). subst.
-    simpl.
-    destruct (funsym_eq_dec
-    (projT1
-       (find_constr_rep gamma_valid m Hinctx (map (val v) vs2)
-          (eq_trans (map_length (val v) vs2)
-             e0)
-          (dom_aux pd) adt Hinmut (adts pd m (map (val v) vs2)) 
-          (gamma_all_unif gamma_valid m Hinctx)
-          (scast (adts pd m (map (val v) vs2) adt Hinmut)
-             (dom_cast (dom_aux pd)
-                (eq_trans eq_refl (v_subst_cons (adt_name adt) vs2)) d))))
-    f); [|reflexivity].
-
-    (*Need nested induction, simplify first*)
-    generalize dependent (find_constr_rep gamma_valid m Hinctx (map (val v) vs2)
-    (eq_trans (map_length (val v) vs2)
-       e0)
-    (dom_aux pd) adt Hinmut (adts pd m (map (val v) vs2)) 
-    (gamma_all_unif gamma_valid m Hinctx)
-    (scast (adts pd m (map (val v) vs2) adt Hinmut)
-       (dom_cast (dom_aux pd)
-          (eq_trans eq_refl (v_subst_cons (adt_name adt) vs2))
-          d))).
-    intros constr. destruct constr as [f' Hf']. simpl. intros Hf; subst.
-    simpl.
-    (*Now remove Hvslen1*)
-    generalize dependent (Hvslen1 m adt vs2 f eq_refl
-    (pat_has_type_valid gamma_valid (Pconstr f vs ps)
-       (vty_cons (adt_name adt) vs2) Hval1) (fst (proj1_sig Hf'))).
-    generalize dependent (Hvslen1 m adt vs2 f eq_refl
-    (pat_has_type_valid gamma_valid (Pconstr f vs ps)
-       (vty_cons (adt_name adt) vs2) Hval2) (fst (proj1_sig Hf'))).
-    intros. assert (e = e1) by (apply UIP_dec, Nat.eq_dec); subst.
-    match goal with
-    | |- (iter_arg_list ?l ?vs2 ?a ?H) = iter_arg_list ?l ?vs2 ?a ?H2 =>
-      generalize dependent H;
-      generalize dependent H2
-    end.
-    destruct Hf'. simpl.
-    destruct x. simpl.
-    generalize dependent (sym_sigma_args_map v f vs2 e1).
-    clear Hval1 Hval2.
-    clear e.
-    unfold sym_sigma_args in *.
-    generalize dependent ps.
-    generalize dependent a.
-    generalize dependent (s_args f).
-    clear.
-    induction l; simpl; intros.
-    + destruct ps; reflexivity.
-    + destruct ps; try reflexivity. simpl.
-      inversion H; subst.
-      rewrite H2 with (Hval2:= (Forall_inv f0)). simpl.
-      rewrite !hlist_tl_cast. 
-      rewrite IHl with(f:=(Forall_inv_tail f0)); auto.
-  - simpl. replace (match_val_single v ty p1 (proj1' (pat_or_inv Hval1)) d) with
-    (match_val_single v ty p1 (proj1' (pat_or_inv Hval2)) d) by apply IHp1.
-    destruct (match_val_single v ty p1 (proj1' (pat_or_inv Hval2)) d); auto.
-  - simpl. rewrite IHp with (Hval2:=(proj1' (pat_bind_inv Hval2))). reflexivity.
 Qed.
 
 (*3. The variables bound are exactly the free variables of pattern p.
@@ -1423,7 +1131,7 @@ Qed.
 
 (*Now we give the denotational semantics:*)
 
-Section Defs.
+Section TermFmlaRep.
 
 Variable vt: val_typevar.
 
@@ -1643,12 +1351,15 @@ with formula_rep (v: val_vars pd vt) (f: formula)
     end Hps Hall in
     match_rep xs Hps Hall.
 
-End Defs.
+End TermFmlaRep.
 
-(*We want these in the rest of the file*)
+End DenotDef.
+
+(*Tactics for proving things about the denotational semantics*)
+
 Ltac simpl_rep :=
   repeat match goal with
-  | |- context [term_rep ?vt ?pf ?v ?t ?ty ?Hty] =>
+  | |- context [term_rep ?valid ?pd ?vt ?pf ?v ?t ?ty ?Hty] =>
     lazymatch t with
     | Tconst (ConstInt ?z) => rewrite term_rep_equation_1
     | Tconst (ConstReal ?r) => rewrite term_rep_equation_2
@@ -1659,7 +1370,7 @@ Ltac simpl_rep :=
     | Tmatch ?t ?v ?ps => rewrite term_rep_equation_7
     | Teps ?f ?v => rewrite term_rep_equation_8
     end
-  | |- context [formula_rep ?vt ?pf ?v ?f ?Hval] =>
+  | |- context [formula_rep ?valid ?pd ?vt ?pf ?v ?f ?Hval] =>
     lazymatch f with
     | Fpred ?p ?vs ?ts => rewrite formula_rep_equation_1
     | Fquant Tforall ?x ?f' => rewrite formula_rep_equation_2
@@ -1693,125 +1404,496 @@ Ltac iter_match_gen Hval Htm Hpat Hty :=
   intros Htm Hpat Hty;
   revert Htm Hpat Hty.
 
-Section Lemmas.
+(*Now we prove theorems about these semantics. The most 
+  important of these are various irrelevance and extensionality 
+  results, allowing us to change or ignore the various parameters
+  of [term_rep] and [formula_rep] in different cases.
+  *)
 
-Variable (pf: pi_funpred gamma_valid pd).
-Notation funs := (funs gamma_valid pd pf).
+Section Theorems.
 
-(*Results about the Denotational Semantics*)
+(*The first set of theorems do not fix the context;
+  they allow us to change the context under certain circumstances*)
 
-(*Most of these results are about equality of the
-  semantics under changes to the proofs/interpretations/valuations.
-  which are needed to define and prove things about 
-  transformations, recursive functions, inductive predicates, etc*)
+Section ChangeContext.
 
-(*In the first batch of lemmas, we fix a [val_typevar]*)
-Section FixedVT.
-
-Variable vt: val_typevar.
-
-(*First, we need to know that the valid typing proof is irrelevant.
-  This is provable without proof irrelevance, though we (indirectly)
-  assume it by using classical logic*)
-
-Lemma term_form_rep_irrel: forall (tm: term) (f: formula),
-  (forall (v: val_vars pd vt) (ty: vty) (Hty1 Hty2:
-    term_has_type gamma tm ty), 
-      term_rep vt pf v tm ty Hty1 = term_rep vt pf v tm ty Hty2) /\
-  (forall (v: val_vars pd vt) (Hval1 Hval2:
-    formula_typed gamma f), 
-      formula_rep vt pf v f Hval1 = formula_rep vt pf v f Hval2).
+(*Extensionality for [arg_list]*)
+Lemma get_arg_list_ext {gamma1 gamma2 pd} (v: val_typevar)
+  (s: fpsym) (vs: list vty) (ts1 ts2: list term) 
+  (reps1: forall (t: term) (ty: vty),
+    term_has_type gamma1 t ty ->
+    domain (dom_aux pd) (v_subst v ty))
+  (reps2: forall (t: term) (ty: vty),
+    term_has_type gamma2 t ty ->
+    domain (dom_aux pd) (v_subst v ty))
+  (Hts: length ts1 = length ts2)
+  (Hreps: forall (i: nat),
+    i < length ts1 ->
+    forall (ty : vty) Hty1 Hty2,
+    reps1 (nth i ts1 tm_d) ty Hty1 = reps2 (nth i ts2 tm_d) ty Hty2)
+  {args: list vty}
+  (Hlents1: length ts1 = length args)
+  (Hlents2: length ts2 = length args)
+  (Hlenvs1 Hlenvs2: length vs = length (s_params s))
+  (Hall1: Forall (fun x => term_has_type gamma1 (fst x) (snd x))
+    (combine ts1 (map (ty_subst (s_params s) vs) args)))
+  (Hall2: Forall (fun x => term_has_type gamma2 (fst x) (snd x))
+    (combine ts2 (map (ty_subst (s_params s) vs) args))):
+  get_arg_list pd v s vs ts1 reps1 Hlents1 Hlenvs1 Hall1 =
+  get_arg_list pd v s vs ts2 reps2 Hlents2 Hlenvs2 Hall2.
 Proof.
-  apply term_formula_ind; intros; simpl_rep; simpl; auto.
-  - destruct c; simpl_rep; simpl;
-    f_equal; apply UIP_dec; apply vty_eq_dec.
-  - f_equal. f_equal. apply UIP_dec; apply vty_eq_dec.
-  - f_equal. apply UIP_dec; apply vty_eq_dec.
-    f_equal. f_equal. f_equal. apply UIP_dec. apply Nat.eq_dec.
-    f_equal. apply get_arg_list_eq.
-    rewrite Forall_forall. intros x Hinx ty' H1 H2.
-    rewrite Forall_forall in H. apply H. assumption.
-  - replace ((term_rep vt pf v0 tm1 (snd v) (proj1' (ty_let_inv Hty1))))
-    with  (term_rep vt pf v0 tm1 (snd v) (proj1' (ty_let_inv Hty2)))
-    by apply H.
-    apply H0.
-  - replace (formula_rep vt pf v f (proj2' (proj2' (ty_if_inv Hty1))))
-    with (formula_rep vt pf v f (proj2' (proj2' (ty_if_inv Hty2))))
-    by apply H.
-    match goal with | |- context [ if ?b then ?x else ?y] => destruct b end.
-    apply H0. apply H1.
-  - (*We need a nested induction here - we have a tactic to help
-      with generalization*)
-    iter_match_gen Hty1 Htm1 Hpat1 Hty1.
-    iter_match_gen Hty2 Htm2 Hpat2 Hty2.
-    induction ps; simpl; intros; auto.
-    destruct a.
-    (*Bulk of work done in [match_val_single_irrel]*)
-    rewrite (H _ _ Hty1 Hty2) at 1. 
-    rewrite match_val_single_irrel with(Hval2:=(Forall_inv Hpat2)).
-    simpl.
-    destruct (match_val_single vt v p 
-      (Forall_inv Hpat2) (term_rep vt pf v0 tm v Hty2)).
-    + inversion H0; subst. apply (H3 (extend_val_with_list pd vt v0 l)).
-    + inversion H0; subst.
-      apply IHps. auto.
-  - f_equal. apply functional_extensionality_dep.
-    intros x.
-    rewrite (H (substi vt v0 v (dom_cast (dom_aux pd)
-    (f_equal (val vt) (proj2' (ty_eps_inv Hty1))) x))
-      (proj1' (ty_eps_inv Hty1))
-    (proj1' (ty_eps_inv Hty2))).
-    assert (proj2' (ty_eps_inv Hty1) =
-    (proj2' (ty_eps_inv Hty2))).
-    apply UIP_dec. apply vty_eq_dec. rewrite H0.
-    reflexivity.
-  - simpl. f_equal. apply get_arg_list_eq.
-    rewrite Forall_forall. intros x Hinx ty' H1 H2.
-    rewrite Forall_forall in H. apply H. assumption.
-  - destruct q; simpl_rep_full;
-    repeat match goal with |- context [ all_dec ?P ] => 
-      destruct (all_dec P); simpl; auto end.
-    + exfalso. apply n. intros d.
-      erewrite (H (substi vt v0 v d)).
-      apply i.
-    + exfalso. apply n. intros d.
-      erewrite H. apply i.
-    + exfalso. apply n. 
-      destruct e as [d Hd].
-      exists d. erewrite H. apply Hd.
-    + exfalso. apply n.
-      destruct e as [d Hd].
-      exists d. erewrite H. apply Hd.
-  - erewrite H. erewrite H0. reflexivity.
-  - erewrite H. erewrite H0. reflexivity.
-  - erewrite H. reflexivity.
-  - erewrite H. erewrite H0. reflexivity.
-  - erewrite H. erewrite H0. erewrite H1. reflexivity.
-  - (*Match case again - proof almost identical*)
-    iter_match_gen Hval1 Htm1 Hpat1 Hty1.
-    iter_match_gen Hval2 Htm2 Hpat2 Hty2.
-    induction ps; simpl; intros; auto.
-    destruct a.
-    (*Bulk of work done in [match_val_single_irrel]*)
-    rewrite (H _ _ Hty1 Hty2) at 1.
-    rewrite match_val_single_irrel with (Hval2:=(Forall_inv Hpat2)); simpl.
-    destruct (match_val_single vt v p (Forall_inv Hpat2) (term_rep vt pf v0 tm v Hty2)).
-    + inversion H0; subst. apply (H3 (extend_val_with_list pd vt v0 l)).
-    + inversion H0; subst.
-      apply IHps. auto.
+  unfold get_arg_list. simpl.
+  assert (Hlenvs1 = Hlenvs2). apply UIP_dec. apply Nat.eq_dec.
+  subst.
+  generalize dependent args.
+  generalize dependent ts2. 
+  induction ts1; simpl; intros. 
+  - destruct ts2; [|subst; inversion Hts].
+    destruct args; auto. inversion Hlents1.
+  - destruct ts2; inversion Hts.
+    destruct args.
+    + inversion Hlents2.
+    + simpl in Hlenvs2. simpl. f_equal.
+      * f_equal.
+        apply (Hreps 0). lia.
+      * apply IHts1; auto.
+        intros j Hj ty Hty1 Hty2.
+        apply (Hreps (S j)); lia.
 Qed.
 
-Definition term_rep_irrel t := proj_tm term_form_rep_irrel t.
-Definition fmla_rep_irrel f := proj_fmla term_form_rep_irrel f.
+(*An alternate, nicer form when ts are equal*)
+Lemma get_arg_list_eq {gamma} pd (v: val_typevar)
+(s: fpsym) (vs: list vty) (ts: list term) 
+(reps1 reps2: forall (t: term) (ty: vty),
+  term_has_type gamma t ty ->
+  domain (dom_aux pd) (v_subst v ty))
+(Hreps: Forall
+(fun tm : term =>
+ forall (ty : vty) (Hty1 Hty2: term_has_type gamma tm ty),
+ reps1 tm ty Hty1 = reps2 tm ty Hty2) ts)
+{args: list vty}
+(Hlents1 Hlents2: length ts = length args)
+(Hlenvs1 Hlenvs2: length vs = length (s_params s))
+(Hall1 Hall2: Forall (fun x => term_has_type gamma (fst x) (snd x))
+  (combine ts (map (ty_subst (s_params s) vs) args))):
+get_arg_list pd v s vs ts reps1 Hlents1 Hlenvs1 Hall1 =
+get_arg_list pd v s vs ts reps2 Hlents2 Hlenvs2 Hall2.
+Proof.
+  apply get_arg_list_ext; auto.
+  intros i Hi ty H1 H2.
+  rewrite Forall_forall in Hreps; apply Hreps.
+  apply nth_In; auto.
+Qed.
 
-End FixedVT.
+Lemma is_vty_adt_same_muts {gamma1 gamma2: context}
+  (Hadts: mut_of_context gamma1 = mut_of_context gamma2)
+  ty:
+  is_vty_adt gamma1 ty = is_vty_adt gamma2 ty.
+Proof.
+  unfold is_vty_adt. destruct ty; auto.
+  assert (find_ts_in_ctx gamma1 t = find_ts_in_ctx gamma2 t). {
+    unfold find_ts_in_ctx. rewrite Hadts. reflexivity.
+  }
+  rewrite H. reflexivity.
+Qed.
+
+(*A similar result for [match_val_single]*)
+Lemma match_val_single_ext {gamma1 gamma2: context}
+  (gamma_valid1: valid_context gamma1)
+  (gamma_valid2: valid_context gamma2)
+  (*The contexts must agree on all ADTs*)
+  (Hadts: mut_of_context gamma1 = mut_of_context gamma2)
+  (pd: pi_dom)
+  (vt: val_typevar) (ty: vty)
+  (p: pattern)
+  (Hval1: pattern_has_type gamma1 p ty)
+  (Hval2: pattern_has_type gamma2 p ty)
+  (d: domain (dom_aux pd) (v_subst vt ty)):
+  match_val_single gamma_valid1 pd vt ty p Hval1 d =
+  match_val_single gamma_valid2 pd vt ty p Hval2 d.
+Proof.
+  revert ty d Hval1 Hval2.
+  induction p; intros; auto.
+  - rewrite !match_val_single_rewrite; simpl.
+    (*The hard case: need lots of generalization for dependent types
+      and need nested induction*) 
+    generalize dependent (@is_vty_adt_some gamma1 ty).
+    generalize dependent (@is_vty_adt_some gamma2 ty).
+    generalize dependent (@adt_vty_length_eq gamma1 gamma_valid1 ty).
+    generalize dependent (@adt_vty_length_eq gamma2 gamma_valid2 ty).
+    generalize dependent (@constr_length_eq gamma1 gamma_valid1 ty).
+    generalize dependent (@constr_length_eq gamma2 gamma_valid2 ty).
+    rewrite (is_vty_adt_same_muts Hadts).
+    destruct (is_vty_adt gamma2 ty) eqn : Hisadt; [|reflexivity].
+    intros Hvslen1_1 Hvslen1_2 Hvslen2_1 Hvslen2_2 Hadtspec1 Hadtspec2.
+    destruct p as [[m adt] vs2].
+    destruct (Hadtspec1 m adt vs2 eq_refl)
+      as [Htyeq1 [Hinmut1 Hinctx1]].
+    destruct (Hadtspec2 m adt vs2 eq_refl)
+      as [Htyeq2 [Hinmut2 Hinctx2]].
+    simpl.
+    (*Some easy equalities*)
+    assert (Hinmut1 = Hinmut2) by apply bool_irrelevance. subst.
+    assert (Htyeq2 = eq_refl). apply UIP_dec. apply vty_eq_dec. subst.
+    generalize dependent  (Hvslen2_2 m adt vs2 eq_refl
+    (pat_has_type_valid gamma_valid1 (Pconstr f vs ps)
+       (vty_cons (adt_name adt) vs2) Hval1)).
+    generalize dependent (Hvslen2_1 m adt vs2 eq_refl
+    (pat_has_type_valid gamma_valid2 (Pconstr f vs ps)
+       (vty_cons (adt_name adt) vs2) Hval2)).
+    intros.
+    assert (e = e0) by (apply UIP_dec; apply Nat.eq_dec). subst.
+    simpl.
+    generalize dependent (gamma_all_unif gamma_valid2 m Hinctx1).
+    generalize dependent  (gamma_all_unif gamma_valid1 m Hinctx2).
+    intros. assert (i = i0) by (apply bool_irrelevance). subst.
+    match goal with
+    | |- match funsym_eq_dec (projT1 ?x) ?f with | left Heq1 => _ | right Hneq1 => _ end =
+      match funsym_eq_dec (projT1 ?y) ?f with | left Heq2 => _ | right Hneq2 => _ end =>
+      assert (projT1 x = projT1 y) by (apply find_constr_rep_change_gamma);
+      destruct x; destruct y; simpl in *; subst
+    end.
+    destruct (funsym_eq_dec x0 f); auto; subst. simpl.
+    (*Now need to show equivalence of s and s0*)
+    destruct s as [[f_in1 a1] Heqa1]; simpl.
+    destruct s0 as [[f_in2 a2] Heqa2]; simpl.
+    simpl in *.
+    assert (f_in2 = f_in1) by (apply bool_irrelevance). subst.
+    (*We can show a1 = a2 by injectivity*)
+    rewrite constr_rep_change_gamma with(gamma_valid2:=gamma_valid2)
+      (m_in2:=Hinctx1) in Heqa1.
+    rewrite Heqa2 in Heqa1.
+    apply constr_rep_inj in Heqa1; auto.
+    subst.
+    (*Now remove Hvslen1*)
+    generalize dependent (Hvslen1_2 m adt vs2 f eq_refl
+    (pat_has_type_valid gamma_valid1 (Pconstr f vs ps)
+       (vty_cons (adt_name adt) vs2) Hval1) f_in1).
+    generalize dependent  (Hvslen1_1 m adt vs2 f eq_refl
+    (pat_has_type_valid gamma_valid2 (Pconstr f vs ps)
+       (vty_cons (adt_name adt) vs2) Hval2) f_in1).
+    intros. assert (e = e1) by (apply UIP_dec, Nat.eq_dec); subst.
+    match goal with
+    | |- (iter_arg_list ?val1 ?pd ?l ?vs2 ?a ?H) = 
+      iter_arg_list ?val2 ?pd ?l ?vs2 ?a ?H2 =>
+      generalize dependent H;
+      generalize dependent H2
+    end.
+    clear Heqa2.
+    generalize dependent (sym_sigma_args_map vt f vs2 e1).
+    clear Hval1 Hval2.
+    clear e0. 
+    unfold sym_sigma_args in *.
+    generalize dependent ps.
+    generalize dependent (s_args f).
+    clear.
+    induction l; simpl; intros.
+    + destruct ps; reflexivity.
+    + destruct ps; try reflexivity. simpl.
+      inversion H; subst.
+      rewrite H2 with (Hval2:= (Forall_inv f0)). simpl.
+      rewrite !hlist_tl_cast. 
+      rewrite IHl with(f:=(Forall_inv_tail f0)); auto.
+  - simpl. rewrite IHp1 with(Hval2:=(proj1' (pat_or_inv Hval2))).
+    rewrite IHp2 with (Hval2:=proj2' (pat_or_inv Hval2)).
+    reflexivity.
+  - simpl. rewrite IHp with (Hval2:=(proj1' (pat_bind_inv Hval2))). 
+    reflexivity.
+Qed.
+
+(*And finally, an extensionality result for terms and formulas:
+  We can change gamma and pf, as long as the interps
+  agree on all function and predicate symbols in the term/
+  formula *)
+Theorem term_fmla_change_gamma_pf {gamma1 gamma2: context}
+(gamma_valid1: valid_context gamma1)
+(gamma_valid2: valid_context gamma2)
+(Hadts: mut_of_context gamma1 = mut_of_context gamma2)
+(pd: pi_dom)
+(pf1: pi_funpred gamma_valid1 pd)
+(pf2: pi_funpred gamma_valid2 pd)
+(vt: val_typevar)
+(t: term) (f: formula):
+(forall (ty: vty) vv
+  (Htty1: term_has_type gamma1 t ty)
+  (Htty2: term_has_type gamma2 t ty)
+  (Hpext: forall p srts a, predsym_in_tm p t -> 
+    preds gamma_valid1 pd pf1 p srts a = 
+    preds gamma_valid2 pd pf2 p srts a)
+  (Hfext: forall f srts a, funsym_in_tm f t ->
+    funs gamma_valid1 pd pf1 f srts a = 
+    funs gamma_valid2 pd pf2 f srts a),
+    term_rep gamma_valid1 pd vt pf1 vv t ty Htty1 =
+    term_rep gamma_valid2 pd vt pf2 vv t ty Htty2
+) /\
+(forall (vv: val_vars pd vt)
+  (Hval1: formula_typed gamma1 f)
+  (Hval2: formula_typed gamma2 f)
+  (Hpext: forall p srts a, predsym_in_fmla p f -> 
+    preds gamma_valid1 pd pf1 p srts a = 
+    preds gamma_valid2 pd pf2 p srts a)
+  (Hfext: forall fs srts a, funsym_in_fmla fs f ->
+    funs gamma_valid1 pd pf1 fs srts a = 
+    funs gamma_valid2 pd pf2 fs srts a),
+  formula_rep gamma_valid1 pd vt pf1 vv f Hval1 =
+  formula_rep gamma_valid2 pd vt pf2 vv f Hval2).
+Proof.
+revert t f; apply term_formula_ind; simpl; intros; simpl_rep_full; auto.
+- destruct c; simpl_rep_full; f_equal; apply UIP_dec; apply vty_eq_dec.
+- f_equal. apply UIP_dec. apply sort_eq_dec.
+- (*Tfun*) 
+  rewrite Hfext by (destruct (funsym_eq_dec f1 f1); auto). 
+  assert ((ty_fun_ind_ret Htty1) = (ty_fun_ind_ret Htty2)).
+  { apply UIP_dec. apply vty_eq_dec. }
+  rewrite H0; clear H0; f_equal.
+  assert ((tfun_params_length Htty1) = (tfun_params_length Htty2)). {
+    apply UIP_dec. apply Nat.eq_dec.
+  }
+  rewrite H0; clear H0; f_equal.
+  f_equal.
+  apply get_arg_list_ext; auto.
+  intros.
+  assert (Hith: In (nth i l1 tm_d) l1). {
+    apply nth_In; auto.
+  }
+  revert H.
+  rewrite Forall_forall; intros.
+  apply H; auto.
+  + intros p srts a Hinp.
+    apply Hpext. apply existsb_exists.
+    exists (nth i l1 tm_d); auto.
+  + intros fs srts a Hinfs.
+    apply Hfext. bool_to_prop. right.
+    exists (nth i l1 tm_d); auto.
+- erewrite H. apply H0; auto.
+  all: intros; try (apply Hfext); try (apply Hpext); simpl;
+  rewrite H1; auto; simpl_bool; auto.
+- rewrite (H _ _ (proj2' (proj2' (ty_if_inv Htty2)))),
+  (H0 _ _ _ (proj1' (ty_if_inv Htty2))),
+  (H1 _ _ _ (proj1' (proj2' (ty_if_inv Htty2)))); auto;
+  intros p srts a Hinp; try (apply Hfext); try (apply Hpext);
+  simpl; rewrite Hinp; simpl_bool; auto.
+- (*match*)
+  iter_match_gen Htty1 Htm1 Hpat1 Hty1.
+  iter_match_gen Htty2 Htm2 Hpat2 Hty2.
+  revert v.
+  induction ps; simpl; intros; auto.
+  destruct a as [pat1 t1]; simpl.
+  rewrite H with(Htty2:=Hty2) at 1.
+  + inversion H0; subst.
+    rewrite match_val_single_ext with(gamma_valid2:=gamma_valid2)
+    (Hval2:=Forall_inv Hpat2); auto. simpl.
+    destruct (match_val_single gamma_valid2 pd vt v pat1 (Forall_inv Hpat2)
+    (term_rep gamma_valid2 pd vt pf2 vv tm v Hty2)) eqn : Hm.
+    * apply H3; intros; [apply Hpext | apply Hfext]; 
+      simpl; rewrite H1; simpl_bool; auto.
+    * apply IHps; auto; intros; [apply Hpext | apply Hfext];
+      simpl; 
+      (*TODO: ugly proof script here*)
+      revert H1; simpl_bool; unfold is_true; intros; solve_bool;
+      revert H1; simpl_bool; auto.
+  + intros. apply Hpext; simpl; rewrite H1; simpl_bool; auto.
+  + intros. apply Hfext; simpl; rewrite H1; simpl_bool; auto.
+- f_equal. repeat (apply functional_extensionality_dep; intros).
+  replace (proj2' (ty_eps_inv Htty1)) with (proj2' (ty_eps_inv Htty2))
+  by (apply UIP_dec; apply vty_eq_dec).
+  erewrite H; [reflexivity | |]; intros;
+  [apply Hpext | apply Hfext]; auto.
+- rewrite Hpext by (destruct (predsym_eq_dec p p); auto). 
+  f_equal.
+  apply get_arg_list_ext; auto.
+  intros.
+  assert (Hith: In (nth i tms tm_d) tms). {
+    apply nth_In; auto.
+  }
+  revert H.
+  rewrite Forall_forall; intros.
+  apply H; auto.
+  + intros ps srts a Hinp.
+    apply Hpext. bool_to_prop. right.
+    exists (nth i tms tm_d); auto.
+  + intros fs srts a Hinfs.
+    apply Hfext. apply existsb_exists.
+    exists (nth i tms tm_d); auto.
+- assert (Hd: forall d,
+    formula_rep gamma_valid1 pd vt pf1 (substi pd vt vv v d) f 
+      (typed_quant_inv Hval1) =
+    formula_rep gamma_valid2 pd vt pf2 (substi pd vt vv v d) f 
+      (typed_quant_inv Hval2)).
+  {
+    intros. apply H; intros; [apply Hpext | apply Hfext]; auto.
+  }
+  destruct q; simpl_rep_full; apply all_dec_eq; split; 
+  try(intros Hall d; specialize (Hall d)); 
+  try (intros [d Hall]; exists d);
+  try rewrite Hd; auto;
+  rewrite <- Hd; auto.
+- rewrite (H _ _ _ (proj1' (typed_eq_inv Hval2))),
+  (H0 _ _ _ (proj2' (typed_eq_inv Hval2))); auto;
+  intros; try apply Hpext; try apply Hfext; rewrite H1; 
+  simpl_bool; auto.
+- rewrite (H _  _ (proj1' (typed_binop_inv Hval2))),
+  (H0 _ _ (proj2' (typed_binop_inv Hval2))); auto;
+  intros; try apply Hpext; try apply Hfext; rewrite H1; 
+  simpl_bool; auto.
+- erewrite H; [reflexivity | |]; intros; [apply Hpext | apply Hfext];
+  auto. 
+- erewrite H. apply H0; auto.
+  all: intros; try (apply Hfext); try (apply Hpext); simpl;
+  rewrite H1; auto; simpl_bool; auto.
+- rewrite (H _ _ (proj1' (typed_if_inv Hval2))),
+  (H0 _ _ (proj1' (proj2' (typed_if_inv Hval2)))),
+  (H1 _ _ (proj2' (proj2' (typed_if_inv Hval2)))); auto;
+  intros p srts a Hinp; try (apply Hfext); try (apply Hpext);
+  simpl; rewrite Hinp; simpl_bool; auto.
+- (*match - exactly the same proof*)
+  iter_match_gen Hval1 Htm1 Hpat1 Hty1.
+  iter_match_gen Hval2 Htm2 Hpat2 Hty2.
+  revert v.
+  induction ps; simpl; intros; auto.
+  destruct a as [pat1 t1]; simpl.
+  rewrite H with(Htty2:=Hty2) at 1.
+  + inversion H0; subst.
+    rewrite match_val_single_ext with(gamma_valid2:=gamma_valid2)
+    (Hval2:=Forall_inv Hpat2); auto. simpl.
+    destruct (match_val_single gamma_valid2 pd vt v pat1 (Forall_inv Hpat2)
+    (term_rep gamma_valid2 pd vt pf2 vv tm v Hty2)) eqn : Hm.
+    * apply H3; intros; [apply Hpext | apply Hfext]; 
+      simpl; rewrite H1; simpl_bool; auto.
+    * apply IHps; auto; intros; [apply Hpext | apply Hfext];
+      simpl; 
+      (*TODO: ugly proof script here*)
+      revert H1; simpl_bool; unfold is_true; intros; solve_bool;
+      revert H1; simpl_bool; auto.
+  + intros. apply Hpext; simpl; rewrite H1; simpl_bool; auto.
+  + intros. apply Hfext; simpl; rewrite H1; simpl_bool; auto.
+Qed.
+
+(*Many useful corollaries from this*)
+
+(*First, change gamma and pf:*)
+
+Definition term_change_gamma_pf {gamma1 gamma2: context}
+(gamma_valid1: valid_context gamma1)
+(gamma_valid2: valid_context gamma2)
+(Hadts: mut_of_context gamma1 = mut_of_context gamma2)
+(pd: pi_dom)
+(pf1: pi_funpred gamma_valid1 pd)
+(pf2: pi_funpred gamma_valid2 pd)
+(t: term)
+(ty: vty)
+(vt: val_typevar):=
+(proj_tm (term_fmla_change_gamma_pf gamma_valid1 gamma_valid2
+Hadts pd pf1 pf2 vt) t) ty.
+
+Definition fmla_change_gamma_pf {gamma1 gamma2: context}
+(gamma_valid1: valid_context gamma1)
+(gamma_valid2: valid_context gamma2)
+(Hadts: mut_of_context gamma1 = mut_of_context gamma2)
+(pd: pi_dom)
+(pf1: pi_funpred gamma_valid1 pd)
+(pf2: pi_funpred gamma_valid2 pd)
+(f: formula)
+(vt: val_typevar):=
+(proj_fmla (term_fmla_change_gamma_pf gamma_valid1 gamma_valid2
+  Hadts pd pf1 pf2 vt) f).
+
+(*Given a fixed gamma, we can change the pf as long as it
+  agrees on all function and predicate symbols in t/f*)
+Corollary tm_change_pf {gamma} (gamma_valid: valid_context gamma)
+  (pd: pi_dom) (p1 p2: pi_funpred gamma_valid pd) 
+  (vt: val_typevar) (v: val_vars pd vt) 
+  (t: term) (ty: vty)
+  (Hty: term_has_type gamma t ty)
+  (Hpext: forall p srts a, predsym_in_tm p t -> 
+    preds gamma_valid pd p1 p srts a = 
+    preds gamma_valid pd p2 p srts a)
+  (Hfext: forall f srts a, funsym_in_tm f t ->
+    funs gamma_valid pd p1 f srts a = 
+    funs gamma_valid pd p2 f srts a):
+  term_rep gamma_valid pd vt p1 v t ty Hty = 
+  term_rep gamma_valid pd vt p2 v t ty Hty.
+Proof.
+  apply term_change_gamma_pf; auto.
+Qed.
+
+Corollary fmla_change_pf {gamma} (gamma_valid: valid_context gamma)
+  (pd: pi_dom) (p1 p2: pi_funpred gamma_valid pd) 
+  (vt: val_typevar) (v: val_vars pd vt) 
+  (f: formula)
+  (Hval: formula_typed gamma f)
+  (Hpext: forall p srts a, predsym_in_fmla p f -> 
+    preds gamma_valid pd p1 p srts a = 
+    preds gamma_valid pd p2 p srts a)
+  (Hfext: forall fs srts a, funsym_in_fmla fs f -> 
+    funs gamma_valid pd p1 fs srts a = 
+    funs gamma_valid pd p2 fs srts a):
+  formula_rep gamma_valid pd vt p1 v f Hval = 
+  formula_rep gamma_valid pd vt p2 v f Hval.
+Proof.
+  apply fmla_change_gamma_pf; auto.
+Qed.
+
+(*Third, given a fixed gamma and pf, our reps
+  are irrelevant in the choice of typing proof
+  (this follows from proof irrelevance, but we do
+  not use it directly)*)
+Corollary match_val_single_irrel {gamma} (gamma_valid: valid_context gamma)
+  (pd: pi_dom) (v: val_typevar) (ty: vty)
+  (p: pattern)
+  (Hval1 Hval2: pattern_has_type gamma p ty)
+  (d: domain (dom_aux pd) (v_subst v ty)) :
+  match_val_single gamma_valid pd v ty p Hval1 d =
+  match_val_single gamma_valid pd v ty p Hval2 d.
+Proof.
+  apply match_val_single_ext; auto.
+Qed.
+
+(*TODO: maybe move corollaries below (after)*)
+
+Corollary term_rep_irrel {gamma} (gamma_valid: valid_context gamma)
+  (pd: pi_dom) (pf: pi_funpred gamma_valid pd)
+  (vt: val_typevar) (vv: val_vars pd vt)
+  (t: term) (ty: vty) (Hty1 Hty2: term_has_type gamma t ty):
+  term_rep gamma_valid pd vt pf vv t ty Hty1 =
+  term_rep gamma_valid pd vt pf vv t ty Hty2.
+Proof.
+  apply term_change_gamma_pf; auto.
+Qed.
+
+Corollary fmla_rep_irrel {gamma} (gamma_valid: valid_context gamma)
+  (pd: pi_dom) (pf: pi_funpred gamma_valid pd)
+  (vt: val_typevar) (vv: val_vars pd vt)
+  (f: formula) (Hval1 Hval2: formula_typed gamma f):
+  formula_rep gamma_valid pd vt pf vv f Hval1 = 
+  formula_rep gamma_valid pd vt pf vv f Hval2.
+Proof.
+  apply fmla_change_gamma_pf; auto.
+Qed.
+
+End ChangeContext.
+
+(*Theorems where the context (and pd) is fixed, but neither pf
+  not any part of the valuation are fixed*)
+
+Section FixedInterp.
+
+Context {gamma: context} (gamma_valid: valid_context gamma)
+  (pd: pi_dom).
+(*TODO: can we fix pf?*)
+Variable (pf: pi_funpred gamma_valid pd).
+Notation funs := (funs gamma_valid pd pf).
+Notation domain := (domain (dom_aux pd)).
+Notation term_rep := (term_rep gamma_valid pd).
+Notation formula_rep := (formula_rep gamma_valid pd).
+Notation match_val_single := (match_val_single gamma_valid pd).
 
 (*Now we prove an extensionality theorem for
-  the val_typevar and val_vars: If we have 2 val_typevars
+  the valuations: If we have 2 val_typevars
   and val_vars which agree on all type variables and free variables,
   respectively, then the term/formula reps agree.
   This is complicated, because the output depends on vt, so we need
-  a cast*)
+  lots of casts. This makes [match_val_single] especially tricky*)
 Section ValExt.
 
 (*Now we need a theorem to tell us what happens if we modify vt, the
@@ -1859,7 +1941,7 @@ Proof.
   apply Hvt.
   eapply fmla_fv_vars_type_vars. apply Hinx. auto.
 Qed.
-  
+    
 Lemma vv_cast_fmla2 {f: formula} {vt1 vt2: val_typevar}
   (vv1: val_vars pd vt1)
   (vv2: val_vars pd vt2)
@@ -1891,6 +1973,101 @@ Proof.
   subst. reflexivity. 
 Qed.
 
+(*Lemma for [get_arg_list] - this is a different extensionality lemma
+  than above (particularly with how reps are handled).
+  This allows us to modify the val_typevar, val_vars, 
+  reps, and proofs.*)
+  
+Lemma get_arg_list_vt_ext (vt1 vt2: val_typevar) (s: fpsym)
+  (vs: list vty) (ts1 ts2: list term) vv1 vv2
+  (reps1 reps2: forall (vt: val_typevar) (pf: pi_funpred gamma_valid pd) 
+    (vv: val_vars pd vt)
+    (t: term) (ty: vty) (Hty: term_has_type gamma t ty),
+    domain (v_subst vt ty))
+  (Hts: length ts1 = length ts2)
+  (Hreps: forall (i: nat),
+    i < length ts1 ->
+    forall (ty: vty) Hty1 Hty2 Heq,
+      dom_cast (dom_aux pd) Heq 
+        (reps1 vt1 pf vv1 (nth i ts1 tm_d) ty Hty1) =
+      reps2 vt2 pf vv2 (nth i ts2 tm_d) ty Hty2)
+  {args: list vty}
+  (Hlents1: length ts1 = length args)
+  (Hlents2: length ts2 = length args)
+  (Hlenvs1 Hlenvs2: length vs = length (s_params s))
+  (Hall1: Forall (fun x => term_has_type gamma (fst x) (snd x))
+    (combine ts1 (map (ty_subst (s_params s) vs) args)))
+  (Hall2: Forall (fun x => term_has_type gamma (fst x) (snd x))
+    (combine ts2 (map (ty_subst (s_params s) vs) args)))
+  (Heq: map (v_subst vt2) vs = map (v_subst vt1) vs):
+  cast_arg_list 
+    (f_equal (fun x => ty_subst_list_s (s_params s) x args) (eq_sym Heq))
+    (get_arg_list pd vt1 s vs ts1 (reps1 vt1 pf vv1) Hlents1 Hlenvs1 Hall1) =
+  get_arg_list pd vt2 s vs ts2 (reps2 vt2 pf vv2) Hlents2 Hlenvs2 Hall2.
+Proof.
+  generalize dependent (f_equal (fun x : list sort => ty_subst_list_s (s_params s) x args) (eq_sym Heq)).
+  clear Heq.
+  unfold get_arg_list. simpl.
+  assert (Hlenvs1 = Hlenvs2). apply UIP_dec. apply Nat.eq_dec.
+  subst.
+  generalize dependent args.
+  generalize dependent ts2. 
+  induction ts1; simpl; intros. 
+  - destruct ts2; [|subst; inversion Hts].
+    destruct args; simpl; auto; [|inversion Hlents1].
+    assert (e = eq_refl). apply UIP_dec. apply list_eq_dec.
+    apply sort_eq_dec. 
+    subst. reflexivity.
+  - destruct ts2; inversion Hts.
+    destruct args.
+    + inversion Hlents2.
+    + simpl in Hlenvs2. simpl.
+      simpl in e.
+      rewrite (cast_arg_list_cons e).
+      f_equal.
+      * rewrite rewrite_dom_cast, !dom_cast_compose.
+        erewrite <- (Hreps 0) with(Hty1:=Forall_inv Hall1) (Heq:=
+        (eq_trans 
+          ((eq_trans (funsym_subst_eq (s_params s) vs vt1 v (s_params_Nodup s) (eq_sym Hlenvs2))
+          (cons_inj_hd e)))
+          (eq_sym ((funsym_subst_eq (s_params s) vs vt2 v (s_params_Nodup s) (eq_sym Hlenvs2)))))
+        ); try lia.
+        rewrite !dom_cast_compose. apply dom_cast_eq.
+      * apply IHts1; auto.
+        intros i Hi ty Hty1 Hty2 Heq.
+        apply (Hreps (S i) (ltac:(lia))).
+Qed.
+
+(*A specialized version of the above without quite as much
+  extensionality in the proofs and with a more convenient 
+  Hreps*)
+Lemma get_arg_list_vt_eq (vt1 vt2: val_typevar) (s: fpsym)
+  (vs: list vty) (ts: list term) vv1 vv2
+  (reps: forall (vt: val_typevar) (pf: pi_funpred gamma_valid pd) 
+    (vv: val_vars pd vt)
+    (t: term) (ty: vty) (Hty: term_has_type gamma t ty),
+    domain (v_subst vt ty))
+  (Hreps: Forall
+    (fun tm : term =>
+      forall (ty: vty) (Hty1 Hty2: term_has_type gamma tm ty) 
+        (Heq: v_subst vt2 ty = v_subst vt1 ty),
+        reps vt1 pf vv1 tm ty Hty1 =
+        dom_cast (dom_aux pd) Heq (reps vt2 pf vv2 tm ty Hty2)
+      ) ts)
+  Hlents Hlenvs Hall
+  (Heq: map (v_subst vt2) vs = map (v_subst vt1) vs):
+  cast_arg_list (f_equal (sym_sigma_args s) (eq_sym Heq))
+    (get_arg_list pd vt1 s vs ts (reps vt1 pf vv1) Hlents Hlenvs Hall) =
+  get_arg_list pd vt2 s vs ts (reps vt2 pf vv2) Hlents Hlenvs Hall.
+Proof.
+  apply get_arg_list_vt_ext; auto. 
+  rewrite Forall_forall in Hreps.
+  intros.
+  symmetry. rewrite Hreps with(Heq:=eq_sym Heq0)(Hty2:=Hty2).
+  rewrite !dom_cast_twice. reflexivity.
+  apply nth_In. auto.
+Qed. 
+  
 (*The two lemmas for [match_val_single]*)
 
 (*First:if we cast d, it does not change whether the
@@ -1912,34 +2089,21 @@ Proof.
     simpl.
     generalize dependent (@is_vty_adt_some gamma ty).
     generalize dependent (@adt_vty_length_eq gamma gamma_valid ty).
-    generalize dependent (@constr_length_eq ty).
+    generalize dependent (@constr_length_eq _ gamma_valid ty).
     destruct (is_vty_adt gamma ty) eqn : Hisadt; [|reflexivity].
     intros Hvslen1 Hvslen2 Hadtspec.
     destruct p as [[m adt] vs2].
     destruct (Hadtspec m adt vs2 eq_refl)
       as [Htyeq [Hinmut Hinctx]].
     simpl.
-     (*This part is actually easy: all nat equality proofs are equal*)
+      (*This part is actually easy: all nat equality proofs are equal*)
     generalize dependent (Hvslen2 m adt vs2 eq_refl
     (pat_has_type_valid gamma_valid (Pconstr f vs ps) ty Hp)).
     intros.
     (*We need to know things about the [find_constr_rep]. *)
-    generalize dependent (find_constr_rep gamma_valid m Hinctx (map (v_subst vt1) vs2)
-      (eq_trans (map_length (v_subst vt1) vs2) e) (dom_aux pd) adt Hinmut
-      (adts pd m (map (v_subst vt1) vs2)) (gamma_all_unif gamma_valid m Hinctx)
-      (scast (adts pd m (map (v_subst vt1) vs2) adt Hinmut)
-         (dom_cast (dom_aux pd)
-            (eq_trans (f_equal (v_subst vt1) Htyeq) (v_subst_cons (adt_name adt) vs2))
-            (dom_cast (dom_aux pd) Heq d)))).
-    generalize dependent (find_constr_rep gamma_valid m Hinctx (map (v_subst vt2) vs2)
-      (eq_trans (map_length (v_subst vt2) vs2) e) (dom_aux pd) adt Hinmut
-      (adts pd m (map (v_subst vt2) vs2)) (gamma_all_unif gamma_valid m Hinctx)
-      (scast (adts pd m (map (v_subst vt2) vs2) adt Hinmut)
-         (dom_cast (dom_aux pd)
-            (eq_trans (f_equal (v_subst vt2) Htyeq) (v_subst_cons (adt_name adt) vs2))
-            d))).
-    intros [f1 [[x_in1 a1] Hcast1]] [f2 [[x_in2 a2] Hcast2]]; simpl.
-    simpl in *. subst. simpl in *.
+    case_find_constr.
+    intros [f1 [[x_in1 a1] Hcast1]] [f2 [[x_in2 a2] Hcast2]]; simpl in *;
+    subst.
     rewrite eq_trans_refl_l in Hcast1, Hcast2. 
     assert (Heq2: map (v_subst vt2) vs2 = map (v_subst vt1) vs2). {
       assert (Heq2:=Heq).
@@ -2013,7 +2177,7 @@ Proof.
     assert ( (cast_arg_list (sym_sigma_args_map vt1 f vs2 e1) a2) =
       cast_arg_list (eq_sym Heq3) 
       (cast_arg_list (sym_sigma_args_map vt2 f vs2 e1)
-     (cast_arg_list (f_equal (sym_sigma_args f) (eq_sym Heq2)) a2))
+      (cast_arg_list (f_equal (sym_sigma_args f) (eq_sym Heq2)) a2))
     ). {
       rewrite !cast_arg_list_compose. apply cast_arg_list_eq.
     }
@@ -2023,8 +2187,8 @@ Proof.
     intros a3. clear H0. clear a2.
     (*Now generalize for induction*)
     match goal with
-    | |- (iter_arg_list ?l ?a1 ?ps ?H = None) <->
-      iter_arg_list ?l ?a2 ?ps ?H = None =>
+    | |- (iter_arg_list ?val ?pd ?l ?a1 ?ps ?H = None) <->
+      iter_arg_list ?val ?pd ?l ?a2 ?ps ?H = None =>
       generalize dependent H
     end.
     (*already use UIP so ok to forget f_equal - need this to
@@ -2078,7 +2242,7 @@ Proof.
     + rewrite IHp in Hmatch. rewrite Hmatch. reflexivity.
     + rewrite <- IHp in Hmatch. rewrite Hmatch. reflexivity.
 Qed.  
-
+  
 (*Part 2: If one (and hence both, by above),
   evaluates to Some l, and the other Some l',
   then each element is equal, up to casting*)
@@ -2109,34 +2273,21 @@ Proof.
     simpl.
     generalize dependent (@is_vty_adt_some gamma ty).
     generalize dependent (@adt_vty_length_eq gamma gamma_valid ty).
-    generalize dependent (@constr_length_eq ty).
+    generalize dependent (@constr_length_eq gamma gamma_valid ty).
     destruct (is_vty_adt gamma ty) eqn : Hisadt; [|discriminate].
     intros Hvslen1 Hvslen2 Hadtspec.
     destruct p as [[m adt] vs2].
     destruct (Hadtspec m adt vs2 eq_refl)
       as [Htyeq [Hinmut Hinctx]].
     simpl.
-     (*This part is actually easy: all nat equality proofs are equal*)
+      (*This part is actually easy: all nat equality proofs are equal*)
     generalize dependent (Hvslen2 m adt vs2 eq_refl
     (pat_has_type_valid gamma_valid (Pconstr f vs ps) ty Hp)).
     intros e.
-    (*We need to know things about the [find_constr_rep].*)
-    generalize dependent (find_constr_rep gamma_valid m Hinctx (map (v_subst vt1) vs2)
-      (eq_trans (map_length (v_subst vt1) vs2) e) (dom_aux pd) adt Hinmut
-      (adts pd m (map (v_subst vt1) vs2)) (gamma_all_unif gamma_valid m Hinctx)
-      (scast (adts pd m (map (v_subst vt1) vs2) adt Hinmut)
-         (dom_cast (dom_aux pd)
-            (eq_trans (f_equal (v_subst vt1) Htyeq) (v_subst_cons (adt_name adt) vs2))
-            (dom_cast (dom_aux pd) Heq d)))).
-    generalize dependent (find_constr_rep gamma_valid m Hinctx (map (v_subst vt2) vs2)
-      (eq_trans (map_length (v_subst vt2) vs2) e) (dom_aux pd) adt Hinmut
-      (adts pd m (map (v_subst vt2) vs2)) (gamma_all_unif gamma_valid m Hinctx)
-      (scast (adts pd m (map (v_subst vt2) vs2) adt Hinmut)
-         (dom_cast (dom_aux pd)
-            (eq_trans (f_equal (v_subst vt2) Htyeq) (v_subst_cons (adt_name adt) vs2))
-            d))).
-    intros [f1 [[x_in1 a1] Hcast1]] [f2 [[x_in2 a2] Hcast2]]; simpl.
-    simpl in *. subst. simpl in *.
+    (*We need to know things about the [find_constr_rep]. *)
+    case_find_constr.
+    intros [f1 [[x_in1 a1] Hcast1]] [f2 [[x_in2 a2] Hcast2]]; simpl in *;
+    subst.
     rewrite eq_trans_refl_l in Hcast1, Hcast2. 
     assert (Heq2: map (v_subst vt2) vs2 = map (v_subst vt1) vs2). {
       assert (Heq2:=Heq).
@@ -2210,7 +2361,7 @@ Proof.
     assert ( (cast_arg_list (sym_sigma_args_map vt1 f vs2 e1) a2) =
       cast_arg_list (eq_sym Heq3) 
       (cast_arg_list (sym_sigma_args_map vt2 f vs2 e1)
-     (cast_arg_list (f_equal (sym_sigma_args f) (eq_sym Heq2)) a2))
+      (cast_arg_list (f_equal (sym_sigma_args f) (eq_sym Heq2)) a2))
     ). {
       rewrite !cast_arg_list_compose. apply cast_arg_list_eq.
     }
@@ -2220,8 +2371,8 @@ Proof.
     intros a3. clear H0. clear a2.
     (*Now generalize for induction*)
     match goal with
-    | |- (iter_arg_list ?l ?a1 ?ps ?H = Some _) ->
-      iter_arg_list ?l ?a2 ?ps ?H = Some _ -> _ =>
+    | |- (iter_arg_list ?val ?pd ?l ?a1 ?ps ?H = Some _) ->
+      iter_arg_list ?val ?pd ?l ?a2 ?ps ?H = Some _ -> _ =>
       generalize dependent H
     end.
     (*already use UIP so ok to forget f_equal - need this to
@@ -2281,7 +2432,7 @@ Proof.
     + destruct (IHp _ _ _ _ _ _ _ Hmatch Hmatch0 x y Hinxy) as [z [Heq1 [Hinxz Hz2]]].
       exists z. exists Heq1. split; auto.
 Qed.
-   
+     
 (*Now we can prove the theorem. This is complicated
   due to all the casting*)
 Theorem tm_fmla_change_vt (t: term) (f: formula):
@@ -2290,7 +2441,7 @@ Theorem tm_fmla_change_vt (t: term) (f: formula):
     (Hvt: forall x, In x (tm_type_vars t) -> vt1 x = vt2 x)
     (Hvv: forall x (Hinx: In x (tm_fv t)) 
       (*NOTE: can use (vv_cast_tm1) for cast, but easier to prove
-        more general*)
+        more general*)                                                                                                                                                                                                                                                                                                                                                                                                                                                                                                                                                                                                                                                                                                                                                                                                                                                                                                                                                                                                                                                                                                                                                                                                                                                                                                                                                                                                                                                                                                                                                                                                                                             
       (Heq: v_subst vt1 (snd x) = v_subst vt2 (snd x)), vv2 x = 
       (dom_cast (dom_aux pd) Heq (vv1 x)))
     (ty: vty)
@@ -2350,12 +2501,10 @@ Proof.
     }
     assert (Hargs: 
     (cast_arg_list (f_equal (sym_sigma_args f1) (eq_sym Hmap)) 
-      (fun_arg_list vt1 f1 l l1 (term_rep vt1 pf vv1) Hty)) =
+      (fun_arg_list pd vt1 f1 l l1 (term_rep vt1 pf vv1) Hty)) =
     
-     (fun_arg_list vt2 f1 l l1 (term_rep vt2 pf vv2) Hty)). {
-      (*Here, we need nested induction - is this enough?*)
+      (fun_arg_list pd vt2 f1 l l1 (term_rep vt2 pf vv2) Hty)). {
       unfold fun_arg_list.
-      (*Need to prove a new lemma*)
       apply get_arg_list_vt_eq.
       revert H.
       rewrite !Forall_forall; intros.
@@ -2374,10 +2523,10 @@ Proof.
     assert (Hfuns: 
     (funs f1 (map (v_subst vt2) l)
     (cast_arg_list (f_equal (sym_sigma_args f1) (eq_sym Hmap))
-       (fun_arg_list vt1 f1 l l1 (term_rep vt1 pf vv1) Hty))) =
+        (fun_arg_list pd vt1 f1 l l1 (term_rep vt1 pf vv1) Hty))) =
     dom_cast (dom_aux pd) (f_equal (funsym_sigma_ret f1) (eq_sym Hmap))
     (funs f1 (map (v_subst vt1) l)
-    (fun_arg_list vt1 f1 l l1 (term_rep vt1 pf vv1) Hty))
+    (fun_arg_list pd vt1 f1 l l1 (term_rep vt1 pf vv1) Hty))
     ).
     { rewrite funs_cast_eq. reflexivity.
     }
@@ -2457,13 +2606,13 @@ Proof.
         rewrite !extend_val_notin; auto.
         - erewrite Hvv. reflexivity.
           simpl. simpl_set; auto.
-        - rewrite <- (match_val_single_free_var vt1). apply n.
+        - rewrite <- (match_val_single_free_var gamma_valid pd vt1). apply n.
           apply Hmatch.
-        - rewrite <- (match_val_single_free_var vt2). apply n.
+        - rewrite <- (match_val_single_free_var gamma_valid pd vt2). apply n.
           apply Hmatch1.
       }
       assert (In x (map fst l0)). {
-        rewrite <- (match_val_single_free_var vt2). apply i.
+        rewrite <- (match_val_single_free_var gamma_valid pd vt2). apply i.
         apply Hmatch1.
       }
       rewrite in_map_iff in H1.
@@ -2547,12 +2696,10 @@ Proof.
     }
     assert (Hargs: 
     (cast_arg_list (f_equal (sym_sigma_args p) (eq_sym Hmap)) 
-      (pred_arg_list vt1 p tys tms (term_rep vt1 pf vv1) Hval)) =
+      (pred_arg_list pd vt1 p tys tms (term_rep vt1 pf vv1) Hval)) =
     
-    (pred_arg_list vt2 p tys tms (term_rep vt2 pf vv2) Hval)). {
-      (*Here, we need nested induction - is this enough?*)
+    (pred_arg_list pd vt2 p tys tms (term_rep vt2 pf vv2) Hval)). {
       unfold pred_arg_list.
-      (*Need to prove a new lemma*)
       apply get_arg_list_vt_eq.
       revert H.
       rewrite !Forall_forall; intros.
@@ -2577,9 +2724,9 @@ Proof.
     }
     assert (forall d1 d2,
       d1 = dom_cast (dom_aux pd) (eq_sym Heq) d2 ->
-      formula_rep vt1 pf (substi vt1 vv1 v d1) f
+      formula_rep vt1 pf (substi pd vt1 vv1 v d1) f
       (typed_quant_inv Hval) =
-      formula_rep vt2 pf (substi vt2 vv2 v d2) f
+      formula_rep vt2 pf (substi pd vt2 vv2 v d2) f
       (typed_quant_inv Hval)).
     {
       intros; subst. apply H; intros.
@@ -2692,13 +2839,13 @@ Proof.
         rewrite !extend_val_notin; auto.
         - erewrite Hvv. reflexivity.
           simpl. simpl_set; auto.
-        - rewrite <- (match_val_single_free_var vt1). apply n.
+        - rewrite <- (match_val_single_free_var gamma_valid pd vt1). apply n.
           apply Hmatch.
-        - rewrite <- (match_val_single_free_var vt2). apply n.
+        - rewrite <- (match_val_single_free_var gamma_valid pd vt2). apply n.
           apply Hmatch1.
       }
       assert (In x (map fst l0)). {
-        rewrite <- (match_val_single_free_var vt2). apply i.
+        rewrite <- (match_val_single_free_var gamma_valid pd vt2). apply i.
         apply Hmatch1.
       }
       rewrite in_map_iff in H1.
@@ -2734,7 +2881,7 @@ Definition tm_change_vt t := proj_tm tm_fmla_change_vt t.
 Definition fmla_change_vt f := proj_fmla tm_fmla_change_vt f.
 
 End ValExt.
-
+  
 Section ValExtCor.
 
 (*From this, we have several corollaries, for which we fix the
@@ -2794,12 +2941,15 @@ Qed.
 
 End ValExtCor.
 
-Section Sub.
+(*Now we fix the val_typevar (we can never fix the val_vars
+  because this changes in each recursive call)*)
+Section FixedVt.
 
-Variable vt: val_typevar.
+Variable (vt: val_typevar).
 
 (*Now prove the substitution theorem for the semantics:
   [[t1[t2/x]]]_v = [[t1]]_(x -> t2, v)*)
+Section Sub.
 
 (*Substitution over [get_arg_list]*)
 Lemma get_arg_list_sub x tm1 s tys tms 
@@ -2819,8 +2969,8 @@ Lemma get_arg_list_sub x tm1 s tys tms
     (combine tms (map (ty_subst (s_params s) tys) (s_args s))))
   (Hall2: Forall (fun x => term_has_type gamma (fst x) (snd x))
     (combine (map (sub_t tm1 x) tms) (map (ty_subst (s_params s) tys) (s_args s)))):
-  get_arg_list vt s tys tms reps1 Hlents1 Hlenvs1 Hall1 =
-  get_arg_list vt s tys (map (sub_t tm1 x) tms) reps2 Hlents2 Hlenvs2 Hall2.
+  get_arg_list pd vt s tys tms reps1 Hlents1 Hlenvs1 Hall1 =
+  get_arg_list pd vt s tys (map (sub_t tm1 x) tms) reps2 Hlents2 Hlenvs2 Hall2.
 Proof.
   apply get_arg_list_ext.
   - rewrite map_length; auto.
@@ -2848,7 +2998,7 @@ Lemma sub_correct (t: term) (f: formula):
       ~ In x (tm_bnd t)),
     term_rep vt pf v (sub_t t1 (x, ty1) t) ty2 Hty3 =
     term_rep vt pf 
-      (substi vt v (x, ty1) (term_rep vt pf v t1 ty1 Hty1))
+      (substi pd vt v (x, ty1) (term_rep vt pf v t1 ty1 Hty1))
       t ty2 Hty2) /\
   (forall (t1: term) (x: string) (ty1: vty)
     (v: val_vars pd vt) 
@@ -2861,7 +3011,7 @@ Lemma sub_correct (t: term) (f: formula):
       ~ In x (fmla_bnd f)),
     formula_rep vt pf v (sub_f t1 (x, ty1) f) Hval3 =
     formula_rep vt pf 
-      (substi vt v (x, ty1) (term_rep vt pf v t1 ty1 Hty1))
+      (substi pd vt v (x, ty1) (term_rep vt pf v t1 ty1 Hty1))
       f Hval2).
 Proof.
   revert t f. apply term_formula_ind; intros; simpl; auto.
@@ -2939,7 +3089,7 @@ Proof.
       types to match*)
     destruct (match_val_single vt v phd (Forall_inv Hpat2)
     (term_rep vt pf
-       (substi vt v0 (x, ty1) (term_rep vt pf v0 t1 ty1 Hty1)) tm v
+       (substi pd vt v0 (x, ty1) (term_rep vt pf v0 t1 ty1 Hty1)) tm v
        Hty2)) as [newval |] eqn : Hmatch.
     + revert Hpat3 Htm3. simpl.
       (*Need to see if (x, ty1) is in the pat_fv of phd*)
@@ -3036,11 +3186,11 @@ Proof.
     vsym_eq (x, ty1) v; intros.
     + (*Need for both cases*)
       assert (Hd: forall d,
-      formula_rep vt pf (substi vt v0 (x, ty1) d) f
+      formula_rep vt pf (substi pd vt v0 (x, ty1) d) f
       (typed_quant_inv Hval3) =
       formula_rep vt pf
-      (substi vt
-        (substi vt v0 (x, ty1) (term_rep vt pf v0 t1 ty1 Hty1))
+      (substi pd vt
+        (substi pd vt v0 (x, ty1) (term_rep vt pf v0 t1 ty1 Hty1))
         (x, ty1) d) f (typed_quant_inv Hval2)).
       {
         intros. rewrite substi_same. apply fmla_rep_irrel.
@@ -3050,11 +3200,11 @@ Proof.
       try (intros [d Hex]; exists d);
       specialize (Hd d); congruence.
     + assert (Hd: forall d,
-      formula_rep vt pf (substi vt v0 v d) 
+      formula_rep vt pf (substi pd vt v0 v d) 
         (sub_f t1 (x, ty1) f) (typed_quant_inv Hval3) =
       formula_rep vt pf
-        (substi vt
-            (substi vt v0 (x, ty1) (term_rep vt pf v0 t1 ty1 Hty1)) v d)
+        (substi pd vt
+            (substi pd vt v0 (x, ty1) (term_rep vt pf v0 t1 ty1 Hty1)) v d)
         f (typed_quant_inv Hval2)).
       {
         intros. rewrite substi_diff; auto.
@@ -3128,7 +3278,7 @@ Proof.
       types to match*)
     destruct (match_val_single vt v phd (Forall_inv Hpat2)
     (term_rep vt pf
-      (substi vt v0 (x, ty1) (term_rep vt pf v0 t1 ty1 Hty1)) tm v
+      (substi pd vt v0 (x, ty1) (term_rep vt pf v0 t1 ty1 Hty1)) tm v
       Hval2)) as [newval |] eqn : Hmatch.
     + revert Hpat3 Htm3. simpl.
       (*Need to see if (x, ty1) is in the pat_fv of phd*)
@@ -3200,6 +3350,7 @@ Definition sub_f_rep f := proj_fmla sub_correct f.
 
 End Sub.
 
+
 Section Wf.
 
 (*If we know that the bound variable names are unique and do
@@ -3260,8 +3411,6 @@ End Wf.
 (*Iterated version of forall, let, and*)
 Section Iter.
 
-Variable vt: val_typevar.
-
 (*Iterated forall*)
 Definition fforalls (vs: list vsymbol) (f: formula) : formula :=
   fold_right (fun x acc => Fquant Tforall x acc) f vs.
@@ -3296,7 +3445,7 @@ Fixpoint substi_mult (vt: val_typevar) (vv: val_vars pd vt)
     (map snd l) -> val_vars pd vt with
   | nil => fun _ => vv
   | x :: tl => fun h' => 
-     (substi_mult vt (substi vt vv x (hlist_hd h')) tl (hlist_tl h')) 
+     (substi_mult vt (substi pd vt vv x (hlist_hd h')) tl (hlist_tl h')) 
   end) vals.
   
 (*And we show that we can use this multi-substitution
@@ -3363,7 +3512,7 @@ val_vars pd vt :=
   | nil => fun _ => vv
   | (v, t) :: tl => fun Hall =>
     substi_multi_let 
-      (substi vt vv v 
+      (substi pd vt vv v 
         (term_rep vt pf vv t (snd v) 
       (Forall_inv Hall))) tl (Forall_inv_tail Hall)
   end Hall.
@@ -3454,8 +3603,6 @@ End Iter.
 
 (*Some other results/transformations we need for IndProp*)
 Section OtherTransform.
-
-Variable vt: val_typevar.
 
 (*true -> P is equivalent to P*)
 Lemma true_impl (vv: val_vars pd vt) (f: formula) (Hval1: formula_typed gamma f)
@@ -3551,7 +3698,7 @@ Proof.
   erewrite fmla_change_vv.
   erewrite (fmla_change_vv vt f2).
   erewrite fmla_rep_irrel.
-  erewrite (fmla_rep_irrel vt f2).
+  erewrite (fmla_rep_irrel gamma_valid pd pf vt _ f2).
   reflexivity.
   all: intros; unfold substi;
   destruct (vsymbol_eq_dec x0 x); subst; auto; try contradiction.
@@ -3579,7 +3726,7 @@ Proof.
   - (*Prove let case here*)
     induction l; auto.
     + simpl; intros; simpl_rep_full. erewrite fmla_rep_irrel.
-      erewrite (fmla_rep_irrel vt f2).
+      erewrite (fmla_rep_irrel gamma_valid pd pf vt _ f2).
       reflexivity.
     + intros. simpl fforalls. erewrite distr_impl_let.
       * rewrite !formula_rep_equation_9. cbv zeta.
@@ -3706,187 +3853,6 @@ Proof.
 Qed.
 
 End OtherTransform.
-
-(*We need to generalize pf below*)
-End Lemmas.
-
-(*Another extensionality lemma:
-  Suppose we have a term/fmla and 2 pi_funpreds which agree
-  on all predicates that are used. Then, their interp is equiv*)
-(*This proof is not interesting, since we never adjust the
-  pre-interp like we do the valuation. We just need to push through
-  the induction*)
-Lemma tm_fmla_change_pf vt (t: term) (f: formula) :
-(forall (p1 p2: pi_funpred gamma_valid pd) 
-  (v: val_vars pd vt) (ty: vty) 
-  (Hty: term_has_type gamma t ty),
-  (forall p srts a, predsym_in_tm p t -> 
-    preds gamma_valid pd p1 p srts a = preds gamma_valid pd p2 p srts a) ->
-  (forall f srts a, funsym_in_tm f t ->
-    funs gamma_valid pd p1 f srts a = funs gamma_valid pd p2 f srts a) ->
-  term_rep vt p1 v t ty Hty = term_rep vt p2 v t ty Hty) /\
-(forall (p1 p2: pi_funpred gamma_valid pd) (v: val_vars pd vt) 
-  (Hval: formula_typed gamma f),
-  (forall p srts a, predsym_in_fmla p f -> 
-    preds gamma_valid pd p1 p srts a = preds gamma_valid pd p2 p srts a) ->
-  (forall fs srts a, funsym_in_fmla fs f -> 
-    funs gamma_valid pd p1 fs srts a = funs gamma_valid pd p2 fs srts a) ->
-  formula_rep vt p1 v f Hval = formula_rep vt p2 v f Hval).
-Proof.
-  revert t f.
-  apply term_formula_ind; intros; simpl_rep_full; auto.
-  - rewrite H1; [|simpl; destruct (funsym_eq_dec f1 f1); auto]. 
-    f_equal. f_equal. f_equal.
-    apply get_arg_list_eq.
-    revert H; rewrite !Forall_forall; intros.
-    rewrite (term_rep_irrel) with(Hty2:=Hty2).
-    apply H; auto.
-    + intros p srts a Hinp.
-      apply H0. simpl. apply existsb_exists. exists x; auto.
-    + intros fs srts a Hinfs.
-      apply H1. simpl. bool_to_prop. right.
-      exists x; auto. 
-  - erewrite H. apply H0; auto.
-    all: intros; try (apply H1); try (apply H2); simpl; rewrite H3; auto;
-    rewrite orb_true_r; auto.
-  - rewrite (H _ p2), (H0 _ p2), (H1 _ p2); auto. 
-    all: intros p srts a Hinp; try (apply H2); try(apply H3); simpl; rewrite Hinp; simpl; auto;
-    rewrite orb_true_r; auto.
-  - (*match*) 
-    iter_match_gen Hty Htm Hpat Hty.
-    revert v0.
-    induction ps; simpl; intros; auto.
-    destruct a as [pat1 t1]; simpl.
-    rewrite H with(p2:=p2) at 1; auto.
-    + destruct (match_val_single vt v pat1 (Forall_inv Hpat) 
-        (term_rep vt p2 v0 tm v Hty)) eqn : Hm.
-      * inversion H0; subst.
-        apply H5; auto.
-        -- intros. apply H1. simpl. rewrite H3; simpl.
-          solve_bool. auto. 
-        -- intros. apply H2. simpl. rewrite H3.
-          solve_bool. auto.
-      * apply IHps; auto.
-        -- inversion H0; subst; auto.
-        -- intros. apply H1. simpl.
-          simpl in H3. unfold is_true. solve_bool.
-          revert H3. simpl_bool. auto.
-        -- intros. apply H2. simpl.
-          simpl in H3. unfold is_true. solve_bool.
-          revert H3. simpl_bool. auto.
-      + intros. apply H1. simpl. rewrite H3; auto.
-      + intros. apply H2. simpl. rewrite H3; auto.
-  - f_equal. apply functional_extensionality_dep.
-    intros. rewrite (H _ p2). reflexivity. all: auto.
-  - rewrite H0; simpl; [|destruct (predsym_eq_dec p p); auto; contradiction].
-    f_equal.
-    apply get_arg_list_eq.
-    revert H; rewrite !Forall_forall; intros.
-    rewrite (term_rep_irrel) with(Hty2:=Hty2).
-    apply H; auto.
-    + intros p' srts a Hinp'.
-      apply H0. simpl. bool_to_prop. right. exists x; auto.
-    + intros f' srts a Hinf'.
-      apply H1. simpl. bool_to_prop. exists x; auto. 
-  - destruct q; simpl_rep_full; apply all_dec_eq.
-    + split; intros Hall d; specialize (Hall d);
-      erewrite H; try apply Hall; auto.
-      intros. rewrite H0; auto.
-      intros. rewrite H1; auto. 
-    + split; intros [d Hall]; exists d;
-      erewrite H; try apply Hall; auto.
-      intros. rewrite H0; auto.
-      intros. rewrite H1; auto.
-  - rewrite (H _ p2), (H0 _ p2). reflexivity.
-    all: intros; try apply H1; try apply H2; simpl; rewrite H3; 
-    simpl_bool; auto.
-  - rewrite (H _ p2), (H0 _ p2). reflexivity.
-    all: intros; try apply H1; try apply H2; simpl; rewrite H3; 
-    simpl_bool; auto.
-  - erewrite H; auto.
-  - erewrite H. apply H0.
-    all: intros; try apply H1; try apply H2; simpl; rewrite H3; 
-    simpl_bool; auto.
-  - rewrite (H _ p2), (H0 _ p2), (H1 _ p2). reflexivity.
-    all: intros; try apply H2; try apply H3; simpl; rewrite H4; 
-    simpl_bool; auto.
-  - (*match*) 
-    iter_match_gen Hval Htm Hpat Hty.
-    revert v0.
-    induction ps; simpl; intros; auto.
-    destruct a as [pat1 f1]; simpl.
-    rewrite H with(p2:=p2) at 1; auto.
-    + destruct (match_val_single vt v pat1 (Forall_inv Hpat) 
-        (term_rep vt p2 v0 tm v Hty)) eqn : Hm.
-      * inversion H0; subst.
-        apply H5; auto.
-        all: intros; try apply H1; try apply H2; simpl; rewrite H3; 
-        simpl_bool; auto.
-      * apply IHps; auto.
-        -- inversion H0; subst; auto.
-        -- intros. apply H1. simpl.
-          simpl in H3. unfold is_true. solve_bool.
-          revert H3; simpl_bool; auto.
-        -- intros. apply H2. simpl.
-          simpl in H3. unfold is_true. solve_bool.
-          revert H3; simpl_bool; auto.
-      + intros. apply H1. simpl. rewrite H3; auto.
-      + intros. apply H2. simpl. rewrite H3; auto.
-Qed.
-
-Definition tm_change_pf vt t := proj_tm (tm_fmla_change_pf vt) t.
-Definition fmla_change_pf vt f := proj_fmla (tm_fmla_change_pf vt) f.
-
-End Denot.
-
-
-(*We give the tactics for other files - TODO: can we
-  reduce duplication?*)
-
-(*We want these in the rest of the file*)
-Ltac simpl_rep :=
-  repeat match goal with
-  | |- context [term_rep ?valid ?pd ?vt ?pf ?v ?t ?ty ?Hty] =>
-    lazymatch t with
-    | Tconst (ConstInt ?z) => rewrite term_rep_equation_1
-    | Tconst (ConstReal ?r) => rewrite term_rep_equation_2
-    | Tvar ?v => rewrite term_rep_equation_3
-    | Tfun ?f ?l1 ?l2 => rewrite term_rep_equation_4
-    | Tlet ?t1 ?v ?t2 => rewrite term_rep_equation_5
-    | Tif ?f ?t1 ?t2 => rewrite term_rep_equation_6
-    | Tmatch ?t ?v ?ps => rewrite term_rep_equation_7
-    | Teps ?f ?v => rewrite term_rep_equation_8
-    end
-  | |- context [formula_rep ?valid ?pd ?vt ?pf ?v ?f ?Hval] =>
-    lazymatch f with
-    | Fpred ?p ?vs ?ts => rewrite formula_rep_equation_1
-    | Fquant Tforall ?x ?f' => rewrite formula_rep_equation_2
-    | Fquant Texists ?x ?f' => rewrite formula_rep_equation_3
-    | Feq ?ty ?t1 ?t2 => rewrite formula_rep_equation_4
-    | Fbinop ?b ?f1 ?f2 => rewrite formula_rep_equation_5
-    | Fnot ?f => rewrite formula_rep_equation_6
-    | Ftrue => rewrite formula_rep_equation_7
-    | Ffalse => rewrite formula_rep_equation_8
-    | Flet ?t ?x ?f' => rewrite formula_rep_equation_9
-    | Fif ?f1 ?f2 ?f3 => rewrite formula_rep_equation_10
-    | Fmatch ?t ?ty1 ?xs => rewrite formula_rep_equation_11
-    end
-  end.
-
-Ltac simpl_rep_full :=
-  repeat (simpl_rep; cbv zeta; simpl).
-
-Ltac iter_match_gen Hval Htm Hpat Hty :=
-  match type of Hval with
-  | term_has_type ?s ?t ?ty =>
-    generalize dependent (proj1' (ty_match_inv Hval));
-    generalize dependent (proj1' (proj2' (ty_match_inv Hval)));
-    generalize dependent (proj2' (proj2' (ty_match_inv Hval)))
-  | formula_typed ?s ?f =>
-    generalize dependent (proj1' (typed_match_inv Hval));
-    generalize dependent (proj1' (proj2' (typed_match_inv Hval)));
-    generalize dependent (proj2' (proj2' (typed_match_inv Hval)))
-  end;
-  clear Hval;
-  intros Htm Hpat Hty;
-  revert Htm Hpat Hty.
+End FixedVt.
+End FixedInterp.
+End Theorems.
