proofs/core/RecFun.v
@@ -504,31 +504,10 @@ Proof.
     (pat_has_type_valid gamma_valid (Pconstr f vs0 ps0) ty Hp)).
     clear Hvslen2.
     intros Hvslen2.
-    destruct (funsym_eq_dec
-    (projT1
-       (find_constr_rep gamma_valid m Hinctx (map (v_subst vt) vs2)
-          (eq_trans (map_length (v_subst vt) vs2) Hvslen2) 
-          (dom_aux pd) adt Hinmut
-          (Interp.adts pd m (map (v_subst vt) vs2)) 
-          (gamma_all_unif gamma_valid m Hinctx)
-          (scast (Interp.adts pd m (map (v_subst vt) vs2) adt Hinmut)
-             (dom_cast (dom_aux pd)
-                (eq_trans (f_equal (v_subst vt) Htyeq)
-                   (v_subst_cons (adt_name adt) vs2)) d)))) f);
+    case_find_constr.
+    intros constr. destruct (funsym_eq_dec (projT1 constr) f);
     [| intros; discriminate].
-    generalize dependent (find_constr_rep gamma_valid m Hinctx (map (v_subst vt) vs2)
-    (eq_trans (map_length (v_subst vt) vs2) Hvslen2) 
-    (dom_aux pd) adt Hinmut
-    (Interp.adts pd m (map (v_subst vt) vs2))
-    (gamma_all_unif gamma_valid m Hinctx)
-    (scast
-       (Interp.adts pd m (map (v_subst vt) vs2) adt Hinmut)
-       (dom_cast (dom_aux pd)
-          (eq_trans (f_equal (v_subst vt) Htyeq)
-             (v_subst_cons (adt_name adt) vs2)) d))).
-    intros constr. destruct constr as [f' Hf']. simpl. intros Hf; subst.
-    simpl.
-    (*generalize dependent ((Hsrtsvalid m adt (adt_name adt) srts f eq_refl Hval (fst (proj1_sig Hf')))).*)
+    destruct constr as [f' Hf']; simpl in *; subst. simpl.
     destruct Hf'. simpl.
     (*Here, let us prove that 
       everything in (snd x) is smaller than d - this is the key
