proofs/proofsystem/NatDed.v
@@ -1,0 +1,805 @@
+(*We give a natural-deduction-style proof system for Why3 goals
+  which is sound by construction.
+  This proof system is purely syntactic, and its use does not
+  require ANY reasoning about typing or the semantics*)
+Require Export Alpha.
+Require Export Task.
+Require Export Util.
+Require Export Shallow.
+Set Bullet Behavior "Strict Subproofs".
+
+
+(*Natural deduction*)
+
+(*Our proof system is very simple:
+  All of the sound transformations can be derived*)
+Inductive derives: task -> Prop :=
+  | D_trans: forall (tr: trans) (t: task) 
+    (l: list task),
+    task_wf t ->
+    sound_trans tr ->
+    tr t = l ->
+    (forall x, In x l -> derives x) ->
+    derives t.
+
+(*Soundness is trivial*)
+Theorem soundness (t: task):
+  derives t ->
+  task_valid t.
+Proof.
+  intros Hd.
+  induction Hd. subst.
+  apply (H0 _ H). subst; auto.
+Qed.
+
+(*Now we give some of the familiar proof rules, as transformations.
+  Some of them we may change to the why3 versions.
+  For each we give the transformation, prove it sound (allowing
+    us to use it outside of the context of this proof system),
+  and then give the derivation version corresponding to the usual
+  natural deduction rules*)
+
+Section NatDed.
+
+(*Axiom rule*)
+Definition axiom_trans (t: task) : list (task) :=
+  if in_bool formula_eq_dec (task_goal t) (task_delta t)
+  then nil else [t].
+
+Lemma axiom_trans_sound : sound_trans axiom_trans.
+Proof.
+  unfold sound_trans, axiom_trans. intros.
+  destruct (in_bool_spec formula_eq_dec (task_goal t) (task_delta t)).
+  - unfold task_valid.
+    split; auto. intros. unfold log_conseq.
+    intros. unfold satisfies in *. intros.
+    specialize (H0 _ i vt vv). 
+    erewrite fmla_rep_irrel. apply H0.
+  - simpl in H. apply H; auto.
+Qed.
+
+(*And now the deduction rule*)
+Theorem D_axiom (t: task) :
+  task_wf t ->
+  In (task_goal t) (task_delta t) ->
+  derives t.
+Proof.
+  intros. eapply (D_trans axiom_trans). auto.
+  apply axiom_trans_sound. 
+  unfold axiom_trans.
+  reflexivity. intros.
+  destruct (in_bool_spec formula_eq_dec (task_goal t) (task_delta t));
+  auto; try contradiction.
+Qed.
+
+(*Weakening*)
+
+(*Remove the first hypothesis*)
+Definition weaken_trans: trans :=
+  fun t =>
+  match task_delta t with
+  | nil => [t]
+  | B :: delta => [mk_task (task_gamma t) delta (task_goal t)]
+  end.
+
+Lemma weaken_trans_sound: sound_trans weaken_trans.
+Proof.
+  unfold sound_trans, weaken_trans. intros.
+  destruct t as [[gam del] goal]. simpl_task.
+  destruct del as [| d1 dtl].
+  - apply H; left; auto.
+  - unfold task_valid. split; auto. intros.
+    specialize (H _ (ltac:(simpl; left; reflexivity))).
+    unfold task_valid in H.
+    destruct H as [Hwf Hval].
+    specialize (Hval gamma_valid Hwf).
+    simpl_task.
+    eapply log_conseq_weaken.
+    erewrite log_conseq_irrel. apply Hval.
+    Unshelve. apply Hwf.
+Qed. 
+
+Theorem D_weaken gamma delta A B:
+  formula_typed gamma A ->
+  derives (gamma, delta, B) ->
+  derives (gamma, A :: delta, B).
+Proof.
+  intros. eapply (D_trans weaken_trans); auto.
+  - inversion H0; subst. destruct H1.
+    constructor; simpl_task; auto.
+  - apply weaken_trans_sound.
+  - intros x [Hx | []]; subst; simpl_task; auto.
+Qed. 
+
+(*And*)
+
+(*And intro*)
+Definition andI_trans : trans :=
+  fun t =>
+  match (task_goal t) with
+  | Fbinop Tand f1 f2 => [task_with_goal t f1; task_with_goal t f2]
+  | _ => [t]
+  end.
+
+Ltac gen_ty :=
+  match goal with
+  | |- is_true (formula_rep ?val ?pd ?vt ?pf ?vv ?goal ?ty) =>
+    generalize dependent ty
+  end.
+
+Lemma andI_trans_sound: sound_trans andI_trans.
+Proof.
+  unfold sound_trans, andI_trans. intros.
+  destruct (task_goal t) eqn : Ht; simpl in H; try solve[apply H; auto].
+  destruct b; simpl in H; try solve[apply H; auto].
+  unfold task_valid. split; auto.
+  intros.
+  unfold log_conseq, satisfies. intros. gen_ty.
+  rewrite Ht. intros. simpl_rep_full.
+  bool_to_prop.
+  split.
+  - specialize (H (task_with_goal t f1) (ltac:(auto))).
+    unfold task_valid, task_with_goal in H; simpl in H.
+    destruct H. specialize (H1 gamma_valid H).
+    unfold log_conseq, satisfies in H1.
+    erewrite fmla_rep_irrel. apply H1; auto.
+    intros. erewrite fmla_rep_irrel. apply H0.
+    Unshelve. auto.
+  - specialize (H (task_with_goal t f2) (ltac:(auto))).
+    unfold task_valid, task_with_goal in H; simpl in H.
+    destruct H. specialize (H1 gamma_valid H).
+    unfold log_conseq, satisfies in H1.
+    erewrite fmla_rep_irrel. apply H1; auto.
+    intros. erewrite fmla_rep_irrel. apply H0.
+    Unshelve. auto.
+Qed.
+
+(*And now the deduction rule*)
+Theorem D_andI gamma (delta: list formula)
+  (f1 f2: formula):
+  derives (gamma, delta, f1) ->
+  derives (gamma, delta, f2) ->
+  derives (gamma, delta, Fbinop Tand f1 f2).
+Proof.
+  intros. eapply (D_trans andI_trans); auto.
+  - inversion H; inversion H0; subst.
+    destruct H1; destruct H6.
+    constructor; simpl; simpl_task; auto.
+    apply closed_binop; auto.
+  - apply andI_trans_sound.
+  - simpl. simpl_task. intros x [Hx | [Hx | []]]; subst; auto.
+Qed.
+ 
+(*And elimination*)
+
+(*To prove A, we can prove A /\ B*)
+Definition andE1_trans (B: formula) : trans :=
+  fun t => [task_with_goal t (Fbinop Tand (task_goal t) B)].
+
+Lemma andE1_trans_sound: forall B, sound_trans (andE1_trans B).
+Proof.
+  intros. unfold sound_trans, andE1_trans.
+  intros. specialize (H _ (ltac:(simpl; left; auto))).
+  destruct t as [[gamma delta] A].
+  unfold task_valid in *; simpl_task.
+  destruct H as [Hwf Hval].
+  split; auto. intros.
+  specialize (Hval gamma_valid Hwf).
+  unfold log_conseq in *.
+  intros. specialize (Hval pd pf pf_full). 
+  prove_hyp Hval.
+  {
+    intros. erewrite satisfies_irrel. apply H. Unshelve. auto.
+  }
+  assert (formula_typed gamma B). {
+    destruct Hwf. simpl_task. destruct task_goal_typed.
+    inversion f_ty; auto.
+  }
+  erewrite satisfies_irrel in Hval.
+  rewrite satisfies_and with (B_ty:=H0) in Hval.
+  apply Hval.
+Qed.
+
+Theorem D_andE1 {gamma delta A B}:
+  derives (gamma, delta, Fbinop Tand A B) ->
+  derives (gamma, delta, A).
+Proof.
+  intros. eapply (D_trans (andE1_trans B)); auto.
+  - inversion H; subst. destruct H0; simpl_task.
+    constructor; auto; simpl_task. apply closed_binop_inv in task_goal_typed.
+    apply task_goal_typed.
+  - apply andE1_trans_sound.
+  - intros x [Hx | []]; subst; auto.
+Qed.
+
+(*And the other elimination rule*)
+
+(*To prove B, we can prove A /\ B*)
+Definition andE2_trans (A: formula) : trans :=
+  fun t => [task_with_goal t (Fbinop Tand A (task_goal t))].
+
+Lemma andE2_trans_sound: forall A, sound_trans (andE2_trans A).
+Proof.
+  intros. unfold sound_trans, andE2_trans.
+  intros. specialize (H _ (ltac:(simpl; left; auto))).
+  destruct t as [[gamma delta] B].
+  unfold task_valid in *; simpl_task.
+  destruct H as [Hwf Hval].
+  split; auto. intros.
+  specialize (Hval gamma_valid Hwf).
+  unfold log_conseq in *.
+  intros. specialize (Hval pd pf pf_full). 
+  prove_hyp Hval.
+  {
+    intros. erewrite satisfies_irrel. apply H. Unshelve. auto.
+  }
+  assert (formula_typed gamma A). {
+    destruct Hwf. simpl_task. destruct task_goal_typed.
+    inversion f_ty; auto.
+  }
+  erewrite satisfies_irrel in Hval.
+  rewrite satisfies_and with (A_ty:=H0) in Hval.
+  apply Hval.
+Qed.
+
+Theorem D_andE2 {gamma delta A B}:
+  derives (gamma, delta, Fbinop Tand A B) ->
+  derives (gamma, delta, B).
+Proof.
+  intros. eapply (D_trans (andE2_trans A)); auto.
+  - inversion H; subst. destruct H0; simpl_task.
+    constructor; auto; simpl_task. apply closed_binop_inv in task_goal_typed.
+    apply task_goal_typed.
+  - apply andE2_trans_sound.
+  - intros x [Hx | []]; subst; auto.
+Qed.
+
+(*Note: prob should do in form for tactic: if H: A /\ B in gamma,
+  then we can instead say that H1 : A and H2 : B in gamma*)
+(*TODO: add once we add names to context*)
+
+(*Implication*)
+
+(*If A, Delta |- B, then Delta |- A -> B*)
+Definition implI_trans: trans :=
+  fun t => 
+  match (task_goal t) with
+  | Fbinop Timplies A B => [mk_task (task_gamma t) (A :: task_delta t) B]
+  | _ => [t]
+  end.
+
+(*Soundness follows directly from the semantic deduction theorem*)
+Lemma implI_trans_sound: sound_trans implI_trans.
+Proof.
+  unfold sound_trans, implI_trans. intros.
+  destruct (task_goal t) eqn : Ht; simpl in H; try solve[apply H; auto].
+  destruct b; simpl in H; try solve[apply H; auto].
+  unfold task_valid. split; auto.
+  intros.
+  destruct t as [[gamma delta] goal]; simpl_task; subst.
+  erewrite log_conseq_irrel.
+  rewrite <- semantic_deduction.
+  specialize (H _ (ltac:(left; reflexivity))).
+  unfold task_valid in H. simpl in H.
+  destruct H.
+  specialize (H0 gamma_valid H).
+  erewrite log_conseq_irrel. apply H0.
+  Unshelve.
+  all: (destruct w_wf; auto;
+    apply closed_binop_inv in task_goal_typed; apply task_goal_typed).
+Qed.
+
+(*And now the deduction rule*)
+Theorem D_implI gamma (delta: list formula) (A B: formula)
+  (*Here, need A to be closed and monomorphic*)
+  (Hc: closed gamma A):
+  derives (gamma, A :: delta, B) ->
+  derives (gamma, delta, Fbinop Timplies A B).
+Proof.
+  intros. eapply (D_trans implI_trans); auto.
+  - inversion H; subst.
+    destruct H0.
+    constructor; auto; simpl_task.
+    + inversion task_delta_typed; auto.
+    + apply closed_binop; auto.
+  - apply implI_trans_sound.
+  - unfold implI_trans. intros. simpl_task.
+    destruct H0 as [Hx | []]; subst; auto.
+Qed.
+
+(*And the implication elimination rule:
+  If Delta |- A -> B and Delta |- A, then Delta |- B*)
+
+(*To prove B, we can prove A -> B and A*)
+Definition implE_trans (A: formula): trans :=
+  fun t =>
+  [task_with_goal t (Fbinop Timplies A (task_goal t));
+    task_with_goal t A].
+
+Lemma implE_trans_sound: forall A, sound_trans (implE_trans A).
+Proof.
+  unfold sound_trans, implE_trans. intros.
+  unfold task_valid. split; auto.
+  intros.
+  assert (E1:=H). assert (E2:=H).
+  specialize (E1 _ (ltac:(simpl; left; reflexivity))).
+  specialize (E2 _ (ltac:(simpl; right; left; reflexivity))).
+  destruct t as [[gamma delta] B].
+  simpl_task. clear H.
+  unfold task_valid in *.
+  destruct E1 as [Hwf1 E1].
+  destruct E2 as [Hwf2 E2]. simpl_task.
+  specialize (E1 gamma_valid Hwf1).
+  specialize (E2 gamma_valid Hwf2).
+  erewrite log_conseq_irrel in E1.
+  rewrite <- semantic_deduction in E1.
+  Unshelve.
+  2: { apply t_wf. } simpl in E1.
+  2: { apply Hwf2. }
+  2: { apply t_wf. } simpl in E1.
+  unfold log_conseq in *; intros.
+  specialize (E1 pd pf pf_full).
+  prove_hyp E1.
+  {
+    intros. destruct Hd; subst.
+    - erewrite satisfies_irrel. apply E2. intros.
+      erewrite satisfies_irrel. apply H. Unshelve. auto.
+    - erewrite satisfies_irrel. apply H. Unshelve. auto.
+  }
+  erewrite satisfies_irrel.
+  apply E1.
+Qed.
+
+(*The derivation form*)
+Theorem D_implE gamma delta A B:
+  derives (gamma, delta, Fbinop Timplies A B) ->
+  derives (gamma, delta, A) ->
+  derives (gamma, delta, B).
+Proof.
+  intros. eapply (D_trans (implE_trans A)); auto.
+  - inversion H; subst.
+    destruct H1. simpl_task.
+    constructor; simpl_task; auto.
+    apply closed_binop_inv in task_goal_typed. apply task_goal_typed.
+  - apply implE_trans_sound.
+  - unfold implE_trans. simpl_task.
+    intros x [Hx | [Hx | []]]; subst; auto.
+Qed.
+
+(*A more useful version: if we can prove
+  that Delta |- A and that Delta, A |- B, then
+  we can prove Delta |- B.
+  This is essentially "assert" in Coq*)
+
+Definition assert_trans (A: formula) : trans :=
+  fun t => [task_with_goal t A;
+    mk_task (task_gamma t) (A :: task_delta t) (task_goal t)].
+
+(*Essentially the same proof*)
+Lemma assert_trans_sound (A: formula) : sound_trans (assert_trans A).
+Proof.
+  unfold sound_trans, implE_trans. intros.
+  unfold task_valid. split; auto.
+  intros.
+  assert (E1:=H). assert (E2:=H).
+  specialize (E1 _ (ltac:(simpl; left; reflexivity))).
+  specialize (E2 _ (ltac:(simpl; right; left; reflexivity))).
+  destruct t as [[gamma delta] B].
+  simpl_task. clear H.
+  unfold task_valid in *.
+  destruct E1 as [Hwf1 E1].
+  destruct E2 as [Hwf2 E2]. simpl_task.
+  specialize (E1 gamma_valid Hwf1).
+  specialize (E2 gamma_valid Hwf2).
+  unfold log_conseq in *; intros.
+  specialize (E2 pd pf pf_full).
+  prove_hyp E2.
+  {
+    intros. destruct Hd; subst.
+    - erewrite satisfies_irrel. apply E1. intros.
+      erewrite satisfies_irrel. apply H. Unshelve. auto.
+    - erewrite satisfies_irrel. apply H. Unshelve. auto.
+  }
+  erewrite satisfies_irrel.
+  apply E2.
+Qed.
+
+(*Derives version*)
+Theorem D_assert gamma delta A B:
+  derives (gamma, delta, A) ->
+  derives (gamma, A :: delta, B) ->
+  derives (gamma, delta, B).
+Proof.
+  intros. eapply (D_trans (assert_trans A)); auto.
+  - inversion H0; subst. destruct H1. simpl_task.
+    constructor; auto. simpl_task.
+    inversion task_delta_typed; auto.
+  - apply assert_trans_sound.
+  - simpl_task. intros x [Hx | [Hx | []]]; subst; auto.
+Qed.
+
+(*As this suggests, we can prove the deduction theorem:
+  Delta |- A -> B iff Delta, A |- B*)
+Theorem derives_deduction gamma delta A B:
+  closed gamma A ->
+  derives (gamma, delta, Fbinop Timplies A B) <->
+  derives (gamma, A :: delta, B).
+Proof.
+  intros.
+  split; intros.
+  2: {
+    apply D_implI; auto.
+  }
+  assert (derives (gamma, A :: delta, Fbinop Timplies A B)). {
+    apply D_weaken; auto. apply H.
+  }
+  assert (derives (gamma, A :: delta, A)). apply D_axiom; simpl; auto.
+  - inversion H0; subst.
+    destruct H2. simpl_task. constructor; auto.
+    simpl_task. constructor; auto.
+    destruct task_goal_typed. inversion f_ty; auto.
+  - apply D_implE with(A:=A); auto.
+Qed.
+
+(*Quantifiers*)
+
+(*Forall intro rule is MUCH harder because we need
+  to modify the context*)
+
+(*If delta |- f [c/x], where c is a fresh constant symbol,
+  then delta |- forall x, f*)
+Definition forallI_trans name : trans :=
+  fun t =>
+  (*Ensure that name does not appear in signature*)
+  if in_bool string_dec name 
+    (map (fun (x: funsym) => s_name x) (sig_f (task_gamma t))) then [t]
+  else
+  match task_goal t with
+  | Fquant Tforall x f => [mk_task 
+    (abs_fun (constsym name (snd x)) :: (task_gamma t))
+    (task_delta t)
+    (safe_sub_f (t_constsym name (snd x)) x f)] 
+  | _ => [t]
+  end.
+
+(*For our proof, we need  a new interpretation where
+  constant symbol c is interpreted as element d*)
+Section InterpWithConst.
+
+Definition funs_with_const {pd} (funs: forall (f : funsym) (srts : list sort),
+arg_list (domain (dom_aux pd)) (sym_sigma_args f srts) ->
+  domain (dom_aux pd) (funsym_sigma_ret f srts))
+(name: string) (s: sort)
+(d: domain (dom_aux pd) s):
+forall (f : funsym) (srts : list sort),
+	       arg_list (domain (dom_aux pd)) (sym_sigma_args f srts) ->
+           domain (dom_aux pd) (funsym_sigma_ret f srts).
+Proof.
+refine (fun f =>
+  match (funsym_eq_dec f (constsym name s)) with
+  | left Heq => fun srts a => _
+  | right _ => funs f
+  end).
+assert (funsym_sigma_ret f srts = s). {
+  rewrite Heq.
+  unfold funsym_sigma_ret. simpl.
+  assert (type_vars s = nil). {
+    destruct s as [ty Hs].
+    unfold is_sort in Hs. simpl. clear -Hs.
+    rewrite null_nil in Hs; auto.
+  }
+  rewrite H. simpl.
+  apply sort_inj; simpl.
+  symmetry.
+  apply subst_is_sort_eq. destruct s; auto.
+}
+exact (dom_cast _ (eq_sym H) d).
+Defined.
+
+Lemma funs_with_const_same {pd} (funs: forall (f : funsym) (srts : list sort),
+arg_list (domain (dom_aux pd)) (sym_sigma_args f srts) ->
+  domain (dom_aux pd) (funsym_sigma_ret f srts))
+(name: string) (s: sort)
+(d: domain (dom_aux pd) s)
+srts a Heq:
+funs_with_const funs name s d (constsym name s) srts a = dom_cast _ Heq d.
+Proof.
+  unfold funs_with_const. destruct (funsym_eq_dec (constsym name s) (constsym name s));
+  try contradiction.
+  apply dom_cast_eq.
+Qed.
+
+Lemma funs_with_const_diff {pd} (funs: forall (f : funsym) (srts : list sort),
+arg_list (domain (dom_aux pd)) (sym_sigma_args f srts) ->
+  domain (dom_aux pd) (funsym_sigma_ret f srts))
+(name: string) (s: sort)
+(d: domain (dom_aux pd) s)
+(f: funsym) srts a:
+f <> constsym name s ->
+funs_with_const funs name s d f srts a = funs f srts a.
+Proof.
+  intros. unfold funs_with_const.
+  destruct (funsym_eq_dec f (constsym name s)); try contradiction; auto.
+Qed.
+
+(*And now we need to prove that this interpretation 
+  still sets the constructors correctly*)
+
+Lemma funs_with_const_constrs {gamma: context} 
+(gamma_valid: valid_context gamma)
+(name: string) (s: sort)
+(gamma_valid': valid_context (abs_fun (constsym name s) :: gamma))
+(pd: pi_dom)
+(pf: pi_funpred gamma_valid pd)
+(d: domain (dom_aux pd) s):
+forall (m : mut_adt) (a : alg_datatype) 
+  (c : funsym) (Hm : mut_in_ctx m gamma) 
+  (Ha : adt_in_mut a m) (Hc : constr_in_adt c a)
+  (srts : list sort)
+  (Hlens : Datatypes.length srts =
+            Datatypes.length (m_params m))
+  (args : arg_list (domain (dom_aux pd))
+            (sym_sigma_args c srts)),
+funs_with_const (funs gamma_valid pd pf) name s d c srts args =
+constr_rep_dom gamma_valid' m Hm srts Hlens
+(dom_aux pd) a Ha c Hc (adts pd m srts) args.
+Proof.
+  intros.
+  rewrite funs_with_const_diff.
+  2: {
+    intro C. subst.
+    assert (~constr_in_adt (constsym name s) a). {
+      apply (proj1 
+        (abs_not_concrete_fun gamma_valid' _ ltac:(simpl; left; auto)) m);
+      auto.
+    }
+    contradiction.
+  }
+  rewrite (constrs _ pd pf m a c Hm Ha Hc srts Hlens).
+  unfold constr_rep_dom.
+  f_equal. f_equal. f_equal. apply UIP_dec. apply sort_eq_dec.
+  apply constr_rep_change_gamma.
+Qed.
+  
+Definition pf_with_const {gamma: context} 
+(gamma_valid: valid_context gamma)
+(name: string) (s: sort)
+(gamma_valid': valid_context (abs_fun (constsym name s) :: gamma))
+(pd: pi_dom)
+(pf: pi_funpred gamma_valid pd)
+(d: domain (dom_aux pd) s):
+pi_funpred gamma_valid' pd :=
+Build_pi_funpred gamma_valid' pd
+  (funs_with_const (funs gamma_valid pd pf) name s d)
+  (preds gamma_valid pd pf)
+  (funs_with_const_constrs gamma_valid name s gamma_valid' pd pf d).
+
+(*This interpretation is still a [full_interp].
+  This is very annoying to show, because the context changes
+  everywhere*)
+Lemma interp_with_const_full {gamma: context} 
+(gamma_valid: valid_context gamma)
+(name: string) (s: sort)
+(gamma_valid': valid_context (abs_fun (constsym name s) :: gamma))
+(pd: pi_dom)
+(pf: pi_funpred gamma_valid pd)
+(pf_full: full_interp gamma_valid pd pf)
+(d: domain (dom_aux pd) s):
+full_interp gamma_valid' pd (pf_with_const gamma_valid name s gamma_valid' pd pf d).
+Proof.
+  destruct pf_full as [full_fun [full_pred [full_ind1 full_ind2]]].
+  (*Key: this constant not used before*)
+  assert (Hconstnew: ~ In (constsym name s) (sig_f gamma)). {
+    inversion gamma_valid'; subst.
+    simpl in H4. inversion H4; subst; auto.
+  }
+  unfold full_interp. split_all; simpl; intros.
+  - rewrite funs_with_const_diff.
+    2: {
+      intro C. subst.
+      assert (~In (constsym name s) (funsyms_of_rec fs)). {
+        apply (abs_not_concrete_fun gamma_valid' _ ltac:(simpl; left; auto)).
+        apply fs_in.
+      }
+      apply in_fun_def in f_in. contradiction.
+    }
+    rewrite (full_fun fs fs_in f args body f_in srts srts_len a vt vv).
+    f_equal. apply UIP_dec. apply sort_eq_dec.
+    apply term_change_gamma_pf; auto.
+    intros.
+    simpl. rewrite funs_with_const_diff; auto.
+    intro C; subst.
+    assert (In (constsym name s) (sig_f gamma)); try contradiction. 
+    eapply term_has_type_funsym_in_sig. 2: apply H.
+    eapply f_body_type; auto. apply fs_in. apply f_in.
+  - (*Predicate very similar*)
+    rewrite (full_pred fs fs_in p args body p_in srts srts_len a vt vv).
+    apply fmla_change_gamma_pf; auto.
+    intros. simpl. rewrite funs_with_const_diff; auto.
+    intro C; subst.
+    assert (In (constsym name s) (sig_f gamma)); try contradiction. 
+    eapply formula_typed_funsym_in_sig. 2: apply H.
+    eapply p_body_type; auto. apply fs_in. apply p_in.
+  - (*First indprop easy*)
+    rewrite fmla_change_gamma_pf with(gamma_valid2:=gamma_valid) 
+      (pf2:=pf) (Hval2:= (indprop_fmla_valid gamma_valid l_in p_in f_in)); auto.
+    intros. simpl. rewrite funs_with_const_diff; auto.
+    intro C; subst.
+    assert (In (constsym name s) (sig_f gamma)); try contradiction. 
+    eapply formula_typed_funsym_in_sig. 2: apply H.
+    eapply indprop_fmla_valid; auto.
+    apply l_in. apply p_in. auto.
+  - (*2nd is a bit harder but similar idea*)
+    eapply full_ind2 with(vt:=vt)(vv:=vv); auto.
+    intros.
+    assert (Hform1 : 
+      Forall (formula_typed (abs_fun (constsym name s) :: gamma)) fs0). {
+      revert Hform. apply Forall_impl. apply formula_typed_expand.
+    }
+    specialize (H _ Hform1 H1).
+    assert ((dep_map
+      (formula_rep gamma_valid pd (vt_with_args vt (s_params p) srts)
+       (interp_with_Ps gamma_valid pd pf (map fst l) Ps) vv) fs0 Hform) =
+    (dep_map
+    (formula_rep gamma_valid' pd (vt_with_args vt (s_params p) srts)
+      (interp_with_Ps gamma_valid' pd
+          (pf_with_const gamma_valid name s gamma_valid' pd pf d) 
+          (map fst l) Ps) vv) fs0 Hform1)).
+    {
+      apply dep_map_ext.
+      intros. apply fmla_change_gamma_pf; simpl; auto;
+      intros.
+      - apply find_apply_pred_ext. auto.
+      - rewrite funs_with_const_diff; auto.
+        intro C; subst.
+        assert (In (constsym name s) (sig_f gamma)); try contradiction. 
+        eapply formula_typed_funsym_in_sig. apply y1. auto.
+    }
+    rewrite H2; auto.
+Qed.    
+
+End InterpWithConst.
+   
+(*Finally, we can prove the transformation sound.
+  It is quite difficult.*)
+Lemma forallI_trans_sound name:
+  sound_trans (forallI_trans name).
+Proof.
+  unfold sound_trans, forallI_trans.
+  intros.
+  destruct (in_bool_spec string_dec name
+  (map (fun x : funsym => s_name x) (sig_f (task_gamma t))));
+  [apply H; simpl; auto|].
+  destruct (task_goal t) eqn : Ht; simpl in H; try solve[apply H; auto].
+  destruct q; simpl in H; try solve[apply H; auto].
+  specialize (H _ (ltac:(left; reflexivity))).
+  destruct t as [[gamma delta] goal];
+  simpl_task; subst.
+  unfold task_valid in *; simpl_task.
+  split; auto.
+  intros.
+  destruct H as [Hwf Hval].
+  assert (Hsort: type_vars (snd v) = nil). {
+    destruct t_wf. simpl_task.
+    destruct task_goal_typed.
+    unfold mono in f_mono. simpl in f_mono.
+    rewrite null_nil in f_mono.
+    apply union_nil in f_mono. apply f_mono.
+  }
+  assert (Hnotused: ~ In (constsym name (snd v)) (sig_f gamma)). {
+    intro C. apply n. rewrite in_map_iff. exists (constsym name (snd v)).
+    split; auto.
+  }
+  assert (Htyval: valid_type gamma (snd v)). {
+    destruct t_wf.
+    simpl_task. destruct task_goal_typed.
+    inversion f_ty; subst. auto.
+  }
+  (*First, prove new context is valid*)
+  assert (gamma_valid': valid_context (abs_fun (constsym name (snd v)) :: gamma)). {
+    constructor; simpl; auto; constructor; auto; try solve[constructor].
+    unfold wf_funsym. simpl. constructor; auto.
+    split.
+    + apply valid_type_expand; auto.
+    + rewrite Hsort; auto.
+  }
+  specialize (Hval gamma_valid' Hwf).
+  (*Now, things get complicated*)
+  unfold log_conseq in *. intros.
+  (*Idea: We assume I |= Delta, want to show I |= forall x, f.
+    First, unfold definition of satisfies*)
+  unfold satisfies. intros.
+  simpl_rep_full.
+  rewrite simpl_all_dec.
+  intros d.
+  (*So we need to show that [[f]]_(x->d, v) holds under interp I
+    and context gamma.
+    To do this, we produce I' for context (c :: gamma)
+    which is the same as I, but sends [[c]] to (v_subst vt (snd v))
+    and sends funs c to d
+    *)
+  destruct v as [vn vty]; simpl in *.
+  assert (Hsort': null (type_vars vty)). {
+    rewrite null_nil; auto.
+  }
+  set (sty := exist _ vty Hsort' : sort).
+  assert (v_subst vt vty = sty).
+  {
+    apply sort_inj; simpl.
+    symmetry. apply subst_is_sort_eq. auto.
+  }
+  (*Annoying dependent type stuff: need to change d to
+    have type domain (dom_aux pd vty)*)
+  set (d' := dom_cast _ H0 d).
+  (*And this is a full interp*)
+  pose proof (interp_with_const_full gamma_valid name sty 
+    gamma_valid' pd pf pf_full d').
+  set (pf' := (pf_with_const gamma_valid name sty gamma_valid' pd pf d')) in *.
+  specialize (Hval pd pf' H1).
+  prove_hyp Hval.
+  {
+    (*Delta is satisfied by pf' because our constant does not
+      appear in any formula in Delta*)
+      intros.
+      rewrite (satisfies_ext gamma_valid' gamma_valid).
+      apply H. Unshelve. all: auto.
+      intros. subst pf'. simpl.
+      rewrite funs_with_const_diff; auto.
+      intro C; subst.
+      assert (In (constsym name vty) (sig_f gamma)); try contradiction.
+      eapply formula_typed_funsym_in_sig.
+      2: apply H2.
+      destruct t_wf.
+      rewrite Forall_forall in task_delta_typed; apply task_delta_typed;
+      auto.
+  }
+  (*Now we know that pf' satisfies f[c/x]*)
+  unfold satisfies in Hval.
+  specialize (Hval vt vv).
+  (*A few typing lemmas*)
+  assert (Hty1: term_has_type (abs_fun (constsym name vty) :: gamma) (t_constsym name vty) vty).
+  {
+    unfold t_constsym.
+    assert (vty = ty_subst (s_params (constsym name vty)) nil (f_ret
+      (constsym name vty))). {
+      simpl. rewrite Hsort. simpl.
+      unfold ty_subst.
+      rewrite <- subst_is_sort_eq; auto.
+    }
+    rewrite H2 at 3.
+    constructor; simpl; auto.
+    apply valid_type_expand; auto.
+    rewrite Hsort; reflexivity.
+  }
+  assert (f_ty: formula_typed gamma f). {
+    destruct w_wf.
+    destruct task_goal_typed. simpl_task.
+    inversion f_ty; auto.
+  }
+  erewrite safe_sub_f_rep with(Hty1:=Hty1) in Hval.
+  (*And now we just have to prove these things equal*)
+  assert ((term_rep gamma_valid' pd vt pf' vv (t_constsym name vty) vty Hty1) = d). {
+    unfold t_constsym. simpl_rep_full.
+    unfold fun_arg_list. simpl.
+    erewrite funs_with_const_same.
+    unfold cast_dom_vty. subst d'. rewrite !dom_cast_compose.
+    apply dom_cast_refl.
+  }
+  rewrite H2 in Hval.
+  (*And now we go from pf' -> pf because d does not appear*)
+  erewrite fmla_change_gamma_pf.
+  apply Hval. all: auto.
+  intros. subst pf'. simpl.
+  rewrite funs_with_const_diff; auto.
+  intro C. subst d'. subst.
+  assert (In (constsym name vty) (sig_f gamma)); try contradiction.
+  eapply formula_typed_funsym_in_sig.
+  apply f_ty. auto.
+  Unshelve.
+  - unfold funsym_sigma_ret. simpl.
+    rewrite Hsort. simpl.  apply sort_inj. simpl.
+    rewrite <- subst_is_sort_eq; auto.
+  - apply formula_typed_expand. auto.
+Qed.
+  
+End NatDed.
