proofs/proofsystem/Shallow.v
@@ -1,0 +1,38 @@
+(*A (very incomplete) shallowly embedded proof system, in which
+  we can represent goals as corresponding goals in Coq.
+  This is incomplete (in part) because of quantifiers: 
+  it is NOT true that [I |= forall x, f] iff forall closed t,
+    [I |= f [t/x]], because there may not be enough closed terms
+  and domain elements may be unmatched. Quantifiers require the
+  context and interpretation to be modified, which we do
+  in our deeply embedded natural deduction proof system.*)
+(*Some of these lemmas are useful for later proofs in NatDed.v*)
+Require Export Logic.
+
+
+(*I |= f1 /\ f2 iff I |= f1 and I |= f2. If only all connectives
+  were so nice*)
+Lemma satisfies_and {gamma} (gamma_valid: valid_context gamma)
+  (pd: pi_dom) (pf: pi_funpred gamma_valid pd)
+  (pf_full: full_interp gamma_valid pd pf)
+  (A B: formula) (A_ty: formula_typed gamma A) 
+  (B_ty: formula_typed gamma B):
+  satisfies gamma_valid pd pf pf_full (Fbinop Tand A B) 
+    (F_Binop _ _ _ _ A_ty B_ty)
+  <-> 
+  satisfies gamma_valid pd pf pf_full A A_ty /\
+  satisfies gamma_valid pd pf pf_full B B_ty.
+Proof.
+  unfold satisfies. split; intros.
+  - split; intros vt vv; specialize (H vt vv); revert H;
+    simpl_rep_full; bool_to_prop; intros [C1 C2]; 
+    erewrite fmla_rep_irrel; [apply C1 | apply C2].
+  - destruct H as [F1 F2]; specialize (F1 vt vv);
+    specialize (F2 vt vv); simpl_rep_full;
+    rewrite fmla_rep_irrel with(Hval2:=A_ty),
+      fmla_rep_irrel with (Hval2:=B_ty), F1, F2; auto.
+Qed.
+
+(*TODO: prove OR, IMPL for closed formulas*)
+
+
