proofs/proofsystem/Util.v
@@ -1,0 +1,65 @@
+Require Export Logic.
+(*utilities to prevent us from having to write the type
+  variables in a function/predicate symbol*)
+
+Definition find_args (l: list vty) : list typevar :=
+  big_union typevar_eq_dec type_vars l.
+
+Lemma find_args_nodup l:
+  nodupb typevar_eq_dec (find_args l).
+Proof.
+  apply (ssrbool.introT (nodup_NoDup _ _)).
+  apply big_union_nodup.
+Qed.
+
+Lemma find_args_check_args_l l1 l2:
+  (forall x, In x l1 -> In x l2) ->
+  check_args (find_args l2) l1.
+Proof.
+  intros.
+  apply (ssrbool.introT (check_args_correct _ _)).
+  intros.
+  unfold find_args, sublist. intros.
+  simpl_set. exists x. split; auto.
+Qed.
+
+Lemma find_args_check_args_in x l:
+  In x l ->
+  check_sublist (type_vars x) (find_args l).
+Proof.
+  intros. apply (ssrbool.introT (check_sublist_correct _ _)).
+  unfold sublist. intros. unfold find_args. simpl_set.
+  exists x; auto.
+Qed.
+
+(*TODO: want to remove proofs from fun, predsym*)
+Definition funsym_noty (name: string) (args: list vty) 
+  (ret: vty) : funsym :=
+  Build_funsym (Build_fpsym name (find_args (ret :: args)) args
+    (find_args_check_args_l _ _ (fun x => in_cons _ x _)) (find_args_nodup _)) 
+    ret (find_args_check_args_in _ _ (in_eq _ _)).
+
+Definition predsym_noty (name: string) (args: list vty) : predsym :=
+  Build_predsym (Build_fpsym name (find_args args) args
+    (find_args_check_args_l _ _ (fun x H => H))
+    (find_args_nodup _)).
+
+(*Constant symbols*)
+
+Definition constsym (name: string) (ty: vty) : funsym :=
+  funsym_noty name nil ty.
+
+Definition t_constsym name s : term :=
+  Tfun (constsym name s) nil nil.
+
+Lemma t_constsym_fv name s:
+  tm_fv (t_constsym name s) = nil.
+Proof.
+  reflexivity.
+Qed.
+
+Lemma t_constsym_mono name s:
+  mono_t (t_constsym name s).
+Proof.
+  reflexivity.
+Qed.
